Bumped lifting.v, depending on refactoring of adequacy into new file

fairis/heap_lang/lifting.v
@@ -4,7 +4,7 @@ From iris.algebra Require Import auth gmap gset excl.
 From iris.base_logic Require Export gen_heap.
 From trillium.prelude Require Import classical_instances.
 From trillium.program_logic Require Export weakestpre adequacy.
-From trillium.fairness Require Export fairness resources fair_termination fairness_finiteness fuel fuel_termination.
+From trillium.fairness Require Export fairness resources fair_termination fuel fuel_termination.
 From trillium.program_logic Require Import ectx_lifting.
 From trillium.fairness.heap_lang Require Export lang.
 From trillium.fairness.heap_lang Require Import tactics notation.
@@ -40,479 +40,8 @@ Proof. solve_inG. Qed.
       (⌜valid_state_evolution_fairness extr auxtr⌝ ∗
        gen_heap_interp (trace_last extr).2.(heap) ∗
        model_state_interp (trace_last extr).1 (trace_last auxtr))%I ;
-    fork_post tid := λ _, tid ↦M ∅;
+    fork_post tid := λ _, (tid ↦M ∅);
 }.
-
-Section adequacy.
-
-Lemma posts_of_empty_mapping `{heapGS Σ M} (e1 e: expr) v (tid : nat) (tp : list expr):
-  tp !! tid = Some e ->
-  to_val e = Some v ->
-  posts_of tp ((λ (_ : val), 0%nat ↦M ∅) ::  (map (λ '(tnew, e), fork_post (locale_of tnew e)) (prefixes_from [e1] (drop (length [e1]) tp)))) -∗
-  tid ↦M ∅.
-Proof.
-  intros Hsome Hval. simpl.
-
-  rewrite (big_sepL_elem_of (λ x, x.2 x.1) _ (v, (λ _: val, tid ↦M ∅)) _) //.
-  apply elem_of_list_omap.
-  exists (e, (λ _: val, tid ↦M ∅)); split; last first.
-  - simpl. apply fmap_Some. exists v. split; done.
-  - destruct tp as [|e1' tp]; first set_solver. simpl.
-    apply elem_of_cons.
-    destruct tid as [|tid]; [left|right]; first by simpl in Hsome; simplify_eq.
-    apply elem_of_lookup_zip_with. eexists tid, e, _. do 2 split =>//.
-    rewrite /locale_of /=.
-    rewrite list_lookup_fmap fmap_Some. simpl in Hsome.
-    exists (e1 :: take tid tp, e). rewrite drop_0. split.
-    + erewrite prefixes_from_lookup =>//.
-    + rewrite /locale_of /= take_length_le //.
-      assert (tid < length tp)%nat; last lia. by eapply lookup_lt_Some.
-Qed.
-
-(* Local Hint Resolve tid_step_tp_length_heap: core. *)
-
-Lemma from_locale_from_lookup tp0 tp tid e :
-  from_locale_from tp0 tp tid = Some e <-> (tp !! (tid - length tp0)%nat = Some e ∧ (length tp0 <= tid)%nat).
-Proof.
-  split.
-  - revert tp0 tid. induction tp as [| e1 tp1 IH]; intros tp0 tid.
-    { unfold from_locale. simpl. done. }
-    unfold from_locale. simpl.
-    destruct (decide (locale_of tp0 e1 = tid)).
-    + intros ?; simplify_eq. rewrite /locale_of /= Nat.sub_diag.
-      split; [done|lia].
-    + intros [H Hlen]%IH. rewrite app_length /= in H.
-      rewrite app_length /= in Hlen.
-      destruct tid as [|tid]; first lia.
-      assert (Heq1 : (length tp0 + 1 = S (length tp0))%nat) by lia.
-      rewrite Heq1 in Hlen.
-      assert (length tp0 ≤ tid)%nat by lia.
-      assert (Heq : (S tid - length tp0)%nat = (S ((tid - (length tp0))))%nat) by lia.
-      rewrite Heq /=. split.
-      * rewrite -H. f_equal. lia.
-      * transitivity tid; try lia. assumption.
-  - revert tp0 tid. induction tp as [|e1 tp1 IH]; intros tp0 tid.
-    { set_solver. }
-    destruct (decide (tid = length tp0)) as [-> | Hneq].
-    + rewrite Nat.sub_diag /=. intros  [? _]. simplify_eq.
-      rewrite decide_True //.
-    + intros [Hlk Hlen]. assert (length tp0 < tid)%nat as Hle by lia.
-      simpl. rewrite decide_False //. apply IH. split.
-      * assert (tid - length tp0 = S ((tid - 1) - length tp0))%nat as Heq by lia.
-        rewrite Heq /= in Hlk. rewrite -Hlk app_length /=. f_equal; lia.
-      * rewrite app_length /=. apply Nat.le_succ_l in Hle. rewrite Nat.add_comm //.
-Qed.
-
-Lemma from_locale_lookup tp tid e :
-  from_locale tp tid = Some e <-> tp !! tid = Some e.
-Proof.
-  assert (from_locale tp tid = Some e <-> (tp !! tid = Some e ∧ 0 ≤ tid)%nat) as H; last first.
-  { split; intros ?; apply H; eauto. split; [done|lia]. }
-  unfold from_locale. replace (tid) with (tid - length (A := expr) [])%nat at 2;
-    first apply from_locale_from_lookup. simpl; lia.
-Qed.
-
-Definition indexes {A} (xs : list A) := imap (λ i _, i) xs.
-
-Lemma locales_of_list_from_indexes (es' es : list expr) :
-  locales_of_list_from es' es = imap (λ i _, length es' + i)%nat es.
-Proof.
-  revert es'. induction es; [done|]; intros es'.
-  rewrite locales_of_list_from_cons=> /=. rewrite /locale_of.
-  f_equiv; [lia|]. rewrite IHes. apply imap_ext.
-  intros x ? Hin. rewrite app_length=> /=. lia.
-Qed.
-
-Lemma locales_of_list_indexes (es : list expr) :
-  locales_of_list es = indexes es.
-Proof. apply locales_of_list_from_indexes. Qed.
-
-Theorem heap_lang_continued_simulation_fair_termination {FM : FairModel}
-        `{FairTerminatingModel FM} {LM:LiveModel heap_lang FM} ξ a1 r1 extr :
-  continued_simulation
-    (sim_rel_with_user LM ξ)
-    ({tr[trfirst extr]}) ({tr[initial_ls (LM := LM) a1 r1]}) →
-  extrace_fairly_terminating extr.
-Proof.
-  apply continued_simulation_fair_termination.
-  - intros ?? contra. inversion contra.
-    simplify_eq. inversion H2.
-  - by intros ex atr [[??]?].
-  - by intros ex atr [[??]?].
-Qed.
-
-Definition rel_always_holds {Σ} `{LM:LiveModel heap_lang M} `{!heapGS Σ LM}
-           (s:stuckness) (ξ : execution_trace heap_lang → finite_trace M
-                  (option $ fmrole M) → Prop) (c1:cfg heap_lang)
-           (c2:live_model_to_model LM) : iProp Σ :=
-  ∀ ex atr c,
-    ⌜valid_system_trace ex atr⌝ -∗
-    ⌜trace_starts_in ex c1⌝ -∗
-    ⌜trace_starts_in atr c2⌝ -∗
-    ⌜trace_ends_in ex c⌝ -∗
-    ⌜∀ ex' atr' oζ ℓ, trace_contract ex oζ ex' →
-                      trace_contract atr ℓ atr' →
-                      ξ ex' (map_underlying_trace atr')⌝ -∗
-    ⌜∀ e2, s = NotStuck → e2 ∈ c.1 → not_stuck e2 c.2⌝ -∗
-    state_interp ex atr -∗
-    posts_of c.1 ((λ _, 0%nat ↦M ∅) :: ((λ '(tnew, e), fork_post (locale_of tnew e)) <$> (prefixes_from c1.1 (drop (length c1.1) c.1)))) -∗
-    |={⊤, ∅}=> ⌜ξ ex (map_underlying_trace atr)⌝.
-
-Theorem strong_simulation_adequacy Σ `(LM:LiveModel heap_lang M)
-    `{!heapGpreS Σ LM} (s: stuckness) (e1 : expr) σ1 (s1: M) (FR: gset _)
-    (ξ : execution_trace heap_lang → finite_trace M (option $ fmrole M) →
-         Prop) :
-  rel_finitary (sim_rel_with_user LM ξ) →
-  live_roles M s1 ≠ ∅ ->
-  (∀ `{Hinv : !heapGS Σ LM},
-    ⊢ |={⊤}=>
-       (* state_interp (trace_singleton ([e1], σ1)) (trace_singleton (initial_ls (LM := LM) s1 0%nat)) ∗ *)
-       ([∗ map] l ↦ v ∈ heap σ1, mapsto l (DfracOwn 1) v) -∗
-       frag_model_is s1 -∗
-       frag_free_roles_are (FR ∖ live_roles _ s1) -∗
-       has_fuels (Σ := Σ) 0%nat (gset_to_gmap (LM.(lm_fl) s1) (M.(live_roles) s1)) ={⊤}=∗
-       WP e1 @ s; locale_of [] e1; ⊤ {{ v, 0%nat ↦M ∅ }} ∗
-       rel_always_holds s ξ ([e1], σ1) (initial_ls (LM := LM) s1 0%nat)) ->
-  continued_simulation (sim_rel_with_user LM ξ) (trace_singleton ([e1], σ1)) (trace_singleton (initial_ls (LM := LM) s1 0%nat)).
-Proof.
-  intros Hfin Hfevol H.
-  apply (wp_strong_adequacy heap_lang LM Σ s); first by eauto.
-  iIntros (?) "".
-  iMod (gen_heap_init (heap σ1)) as (genheap)" [Hgen [Hσ _]]".
-  iMod (model_state_init s1) as (γmod) "[Hmoda Hmodf]".
-  iMod (model_mapping_init s1) as (γmap) "[Hmapa Hmapf]".
-  iMod (model_fuel_init s1) as (γfuel) "[Hfuela Hfuelf]".
-  iMod (model_free_roles_init s1 (FR ∖ live_roles _ s1)) as (γfr) "[HFR Hfr]".
-  set (distG :=
-         {|
-          heap_fairnessGS := {|
-                              fairness_model_name := γmod;
-                              fairness_model_mapping_name := γmap;
-                              fairness_model_fuel_name := γfuel;
-                              fairness_model_free_roles_name := γfr;
-                              |}
-         |}).
-  iMod (H distG) as "Hwp". clear H.
-  iExists state_interp, (λ _, 0%nat ↦M ∅)%I, fork_post.
-  iSplitR.
-  { unfold config_wp. iIntros "!>!>" (???????) "?". done. }
-  (* iAssert (state_interp with "[Hgen Hmoda Hmodf Hmapa Hfuela HFR] Hfr [Hfuelf Hmapf]"). *)
-  (* { iFrame "Hmodf". unfold state_interp. simpl. iFrame. iExists {[ 0%nat := (live_roles Mdl s1) ]}, _. *)
-  (*   iSplitL "Hfuela"; first by rewrite /auth_fuel_is /= fmap_gset_to_gmap //. *)
-  (*   iSplitL "Hmapa"; first by rewrite /auth_mapping_is /= map_fmap_singleton //. *)
-  (*   iSplit; first done. *)
-  (*   iSplit; iPureIntro; [|split]. *)
-  (*   - intros ρ tid. rewrite lookup_gset_to_gmap_Some. *)
-  (*     setoid_rewrite lookup_singleton_Some. split; naive_solver. *)
-  (*   - intros tid Hlocs. rewrite lookup_singleton_ne //. compute in Hlocs. set_solver. *)
-  (*   - rewrite dom_gset_to_gmap. set_solver. } *)
-  iSpecialize ("Hwp" with "Hσ Hmodf Hfr [Hfuelf Hmapf]").
-  { rewrite /has_fuels /frag_mapping_is /= map_fmap_singleton. iFrame.
-    iAssert ([∗ set] ρ ∈ live_roles M s1, ρ ↦F (LM.(lm_fl) s1))%I with "[Hfuelf]" as "H".
-    - unfold frag_fuel_is. setoid_rewrite map_fmap_singleton.
-      rewrite -big_opS_own //. iApply (own_proper with "Hfuelf").
-      rewrite -big_opS_auth_frag. f_equiv. rewrite gset_to_gmap_singletons //.
-    - rewrite dom_gset_to_gmap. iFrame.
-      iApply (big_sepS_mono with "H"). iIntros (ρ Hin) "H".
-      iExists _. iFrame. iPureIntro. apply lookup_gset_to_gmap_Some. done. }
-  iDestruct "Hwp" as ">[Hwp H]".
-  iModIntro. iFrame "Hwp".
-  iSplitL "Hgen Hmoda Hmapa Hfuela HFR".
-  { unfold state_interp. simpl. iFrame. iExists {[ 0%nat := (live_roles M s1) ]}, _.
-    iSplitL "Hfuela"; first by rewrite /auth_fuel_is /= fmap_gset_to_gmap //.
-    iSplitL "Hmapa"; first by rewrite /auth_mapping_is /= map_fmap_singleton //.
-    iSplit; first done.
-    iSplit; iPureIntro; [|split].
-    - intros ρ tid. rewrite lookup_gset_to_gmap_Some.
-      setoid_rewrite lookup_singleton_Some. split; naive_solver.
-    - intros tid Hlocs. rewrite lookup_singleton_ne //. compute in Hlocs. set_solver.
-    - rewrite dom_gset_to_gmap. set_solver. }
-  iIntros (ex atr c Hvalex Hstartex Hstartatr Hendex Hcontr Hstuck Hequiv) "Hsi Hposts".
-  assert ( ∀ (ex' : finite_trace (cfg heap_lang) (olocale heap_lang)) (atr' : auxiliary_trace LM) (oζ : olocale heap_lang) (ℓ : mlabel LM),
-   trace_contract ex oζ ex' → trace_contract atr ℓ atr' → ξ ex' (map_underlying_trace atr')) as Hcontr'.
-  { intros ex' atr' oζ ℓ H1 H2. cut (sim_rel_with_user LM ξ ex' atr'); eauto. rewrite /sim_rel_with_user. intros [??]. done. }
-  iSpecialize ("H" $! ex atr c Hvalex Hstartex Hstartatr Hendex Hcontr' Hstuck).
-  unfold sim_rel_with_user.
-  iAssert (|={⊤}=> ⌜ξ ex (map_underlying_trace atr)⌝ ∗ state_interp ex atr ∗ posts_of c.1
-               ((λ _ : language.val heap_lang, 0%nat ↦M ∅)
-                :: ((λ '(tnew, e), fork_post (language.locale_of tnew e)) <$>
-                    prefixes_from [e1] (drop (length [e1]) c.1))))%I with "[Hsi H Hposts]" as "H".
-  { iApply fupd_plain_keep_l. iFrame. iIntros "[Hsi Hposts]".
-    iSpecialize ("H" with "Hsi Hposts").
-    by iApply fupd_plain_mask_empty. }
-  iMod "H" as "[H1 [Hsi Hposts]]".
-  destruct ex as [c'|ex' tid (e, σ)].
-  - (* We need to prove that the initial state satisfies the property *)
-    destruct atr as [δ|???]; last by inversion Hvalex. simpl.
-    have Heq1 := trace_singleton_ends_in_inv _ _ Hendex.
-    have Heq3 := trace_singleton_starts_in_inv _ _ Hstartex.
-    have Heq4 := trace_singleton_starts_in_inv _ _ Hstartex.
-    pose proof (trace_singleton_starts_in_inv _ _ Hstartatr). simpl.
-    simplify_eq.
-    iApply (fupd_mask_weaken ∅); first set_solver. iIntros "_ !>".
-    assert (∀ (ρ : fmrole M) (tid : nat),
-               ls_mapping (initial_ls (LM := LM) s1 0%nat) !! ρ = Some tid →
-               is_Some (([e1], σ1).1 !! tid)) as HA.
-    { simpl. intros ρ tid Hsome. apply lookup_gset_to_gmap_Some in Hsome as [??].
-      simplify_eq. by eexists _. }
-    iSplit; last done. iClear "H1".
-    iSplit; first done.
-    destruct (to_val e1) as [v1|] eqn:Heq.
-    + iSplit.
-      { iPureIntro. intros ρ tid Hinit.
-        simpl in *. apply lookup_gset_to_gmap_Some in Hinit as [_ <-].
-        rewrite /from_locale //. }
-      iIntros (tid e Hsome Hnoval ρ). destruct tid; last done.
-      simpl in Hsome. compute in Hsome. simplify_eq. simpl.
-      iAssert (0%nat ↦M ∅) with "[Hposts]" as "Hem".
-      { rewrite /= Heq /fmap /=. by iDestruct "Hposts" as "[??]". }
-      iDestruct "Hsi" as "(_&_&Hsi)".
-      iDestruct "Hsi" as "(%m&%FR'&Hfuela&Hmapa&HFR&%Hinvmap&%Hsmall&Hmodel&HfrFR)".
-      iDestruct (frag_mapping_same 0%nat m with "[Hmapa] Hem") as "%H"; first done.
-      iPureIntro. by eapply no_locale_empty.
-    + iSplit; iPureIntro.
-      { simpl. intros ρ tid Hsome. apply lookup_gset_to_gmap_Some in Hsome as [??].
-        simplify_eq. by eexists _. }
-      intros tid e Hsome Hval' ρ.
-      destruct tid as [|tid]; rewrite /from_locale /= in Hsome; by simplify_eq.
-  - (* We need to prove that that the property is preserved *)
-    destruct atr as [|atr' ℓ δ]; first by inversion Hvalex.
-    (* rewrite (trace_singleton_ends_in_inv _ _ Hendex); last exact unit. *)
-    specialize (Hcontr ex' atr' tid ℓ).
-    have H: trace_contract (trace_extend ex' tid (e, σ)) tid ex' by eexists.
-    have H': trace_contract (trace_extend atr' ℓ δ) ℓ atr' by eexists.
-    specialize (Hcontr H H') as Hvs. clear H H' Hcontr.
-    (* destruct Hvalex as (Hlm & Hlt & Hts). *)
-    have H: trace_ends_in ex' (trace_last ex') by eexists.
-    have H': trace_ends_in atr' (trace_last atr') by eexists.
-    iApply (fupd_mask_weaken ∅); first set_solver. iIntros "_ !>".
-    apply (trace_singleton_ends_in_inv (L := unit)) in Hendex.
-    simpl in *. simplify_eq.
-    iDestruct "Hsi" as "((%&%&%Htids)&_&Hsi)".
-    iDestruct "Hsi" as "(%m&%&Hfuela&Hmapa&?&%Hinvmap&%Hsmall&Hmodel&?)".
-    iSplit; [|done].
-    iSplit; [done|].
-    iSplit.
-    + iPureIntro. intros ρ tid' Hsome. simpl. unfold tids_smaller in Htids. eapply Htids. done.
-    + iIntros (tid' e' Hsome Hnoval ρ). simpl.
-      iAssert (tid' ↦M ∅) with "[Hposts]" as "H".
-      { destruct (to_val e') as [?|] eqn:Heq; last done.
-        iApply posts_of_empty_mapping => //.
-        apply from_locale_lookup =>//. }
-      iDestruct (frag_mapping_same tid' m with "Hmapa H") as "%Hlk".
-      { rewrite /auth_mapping_is. iPureIntro. by eapply no_locale_empty. }
-Qed.
-
-Theorem simulation_adequacy Σ `(LM:LiveModel heap_lang M) `{!heapGpreS Σ LM} (s: stuckness) (e1 : expr) σ1 (s1: M) (FR: gset _):
-  (* The model has finite branching *)
-  rel_finitary (sim_rel LM) →
-  live_roles M s1 ≠ ∅ ->
-  (* The initial configuration satisfies certain properties *)
-  (* A big implication, and we get back a Coq proposition *)
-  (* For any proper Aneris resources *)
-  (∀ `{!heapGS Σ LM},
-      ⊢ |={⊤}=>
-        frag_model_is s1 -∗
-        frag_free_roles_are (FR ∖ live_roles _ s1) -∗
-        has_fuels (Σ := Σ) 0%nat (gset_to_gmap (LM.(lm_fl) s1) (M.(live_roles) s1))
-        ={⊤}=∗ WP e1 @ s; 0%nat; ⊤ {{ v, 0%nat ↦M ∅ }}
-  ) ->
-  (* The coinductive pure coq proposition given by adequacy *)
-  @continued_simulation
-    heap_lang
-    LM
-    (sim_rel LM)
-    (trace_singleton ([e1], σ1))
-    (trace_singleton (initial_ls (LM := LM) s1 0%nat)).
-Proof.
-  intros Hfevol Hne H.
-  assert (sim_rel LM = sim_rel_with_user LM (λ _ _, True)) as Heq.
-  { Require Import Coq.Logic.FunctionalExtensionality.
-    Require Import Coq.Logic.PropExtensionality.
-    do 2 (apply functional_extensionality_dep; intros ?).
-    apply propositional_extensionality.
-    unfold sim_rel_with_user. intuition. }
-
-  rewrite Heq.
-  apply (strong_simulation_adequacy Σ LM s _ _ _ FR) =>//.
-  { rewrite -Heq. done. }
-  iIntros (Hinv) "".
-  iPoseProof (H Hinv) as ">H". iModIntro. iIntros "Hσ Hm Hfr Hf". iSplitR "".
-  - iApply ("H" with "Hm Hfr Hf").
-  - iIntros "!>%%%????????". iApply (fupd_mask_weaken ∅); first set_solver. by iIntros "_ !>".
-Qed.
-
-Theorem simulation_adequacy_inftraces Σ `(LM: LiveModel heap_lang M)
-        `{!heapGpreS Σ LM} (s: stuckness) FR
-        e1 σ1 (s1: M)
-        (iex : inf_execution_trace heap_lang)
-        (Hvex : valid_inf_exec (trace_singleton ([e1], σ1)) iex)
-  :
-  (* The model has finite branching *)
-  rel_finitary (sim_rel LM)  →
-  live_roles M s1 ≠ ∅ ->
-  (∀ `{!heapGS Σ LM},
-      ⊢ |={⊤}=>
-     frag_model_is s1 -∗
-         frag_free_roles_are (FR ∖ live_roles _ s1) -∗
-         has_fuels (Σ := Σ) 0%nat (gset_to_gmap (LM.(lm_fl) s1) (M.(live_roles) s1))
-        ={⊤}=∗ WP e1 @ s; 0%nat; ⊤ {{ v, 0%nat ↦M ∅ }}
-  ) ->
-  (* The coinductive pure coq proposition given by adequacy *)
-  exists iatr,
-  @valid_inf_system_trace _ LM
-    (@continued_simulation
-       heap_lang
-       LM
-       (sim_rel LM))
-    (trace_singleton ([e1], σ1))
-    (trace_singleton (initial_ls (LM := LM) s1 0%nat))
-    iex
-    iatr.
-Proof.
-  intros Hfin Hlr Hwp.
-  eexists.
-  eapply produced_inf_aux_trace_valid_inf.
-  Unshelve.
-  - econstructor.
-  - apply (simulation_adequacy Σ LM s _ _ _ FR) => //.
-  - done.
-Qed.
-
-Definition heap_lang_extrace : Type := extrace heap_lang.
-
-Theorem simulation_adequacy_traces Σ `(LM : LiveModel heap_lang M) `{!heapGpreS Σ LM} (s: stuckness) FR
-        e1 (s1: M)
-        (extr : heap_lang_extrace)
-        (Hvex : extrace_valid extr)
-        (Hexfirst : (trfirst extr).1 = [e1])
-  :
-  (* The model has finite branching *)
-  rel_finitary (sim_rel LM) →
-  live_roles M s1 ≠ ∅ ->
-  (∀ `{!heapGS Σ LM},
-      ⊢ |={⊤}=>
-        frag_model_is s1 -∗
-         frag_free_roles_are (FR ∖ live_roles _ s1) -∗
-         has_fuels (Σ := Σ) 0%nat (gset_to_gmap (LM.(lm_fl) s1) (M.(live_roles) s1))
-        ={⊤}=∗ WP e1 @ s; 0%nat; ⊤ {{ v, 0%nat ↦M ∅ }}
-  ) ->
-  (* The coinductive pure coq proposition given by adequacy *)
-  ∃ (auxtr : auxtrace LM), exaux_traces_match extr auxtr.
-Proof.
-  intros Hfin Hlr Hwp.
-  have [iatr Hbig] : exists iatr,
-      @valid_inf_system_trace
-        heap_lang LM
-        (@continued_simulation
-           heap_lang
-           LM
-           (sim_rel LM))
-        (trace_singleton ([e1], (trfirst extr).2))
-        (trace_singleton (initial_ls (LM := LM) s1 0%nat))
-        (from_trace extr)
-        iatr.
-  { apply (simulation_adequacy_inftraces _ _ s FR); eauto.
-    eapply from_trace_preserves_validity; eauto; first econstructor.
-    simpl. destruct (trfirst extr) eqn:Heq.
-    simpl in Hexfirst. rewrite -Hexfirst Heq //. }
-  exists (to_trace (initial_ls (LM := LM) s1 0%nat) iatr).
-  eapply (valid_inf_system_trace_implies_traces_match (continued_simulation (sim_rel LM))); eauto.
-  - by intros ? ? [? ?]%continued_simulation_rel.
-  - by intros ? ? [? ?]%continued_simulation_rel.
-  - apply from_trace_spec. simpl. destruct (trfirst extr) eqn:Heq. simplify_eq. f_equal.
-    simpl in Hexfirst. rewrite -Hexfirst Heq //.
-  - apply to_trace_spec.
-Qed.
-
-Theorem simulation_adequacy_model_trace Σ `(LM : LiveModel heap_lang M)
-        `{!heapGpreS Σ LM} (s: stuckness) FR
-        e1 (s1: M)
-        (extr : heap_lang_extrace)
-        (Hvex : extrace_valid extr)
-        (Hexfirst : (trfirst extr).1 = [e1])
-  :
-  (* The model has finite branching *)
-  rel_finitary (sim_rel LM) →
-  live_roles M s1 ≠ ∅ ->
-  (∀ `{!heapGS Σ LM},
-      ⊢ |={⊤}=>
-        frag_model_is s1 -∗
-         frag_free_roles_are (FR ∖ live_roles _ s1) -∗
-         has_fuels (Σ := Σ) 0%nat (gset_to_gmap (LM.(lm_fl) s1) (M.(live_roles) s1))
-        ={⊤}=∗ WP e1 @ s; 0%nat; ⊤ {{ v, 0%nat ↦M ∅ }}
-  ) ->
-  (* The coinductive pure coq proposition given by adequacy *)
-  ∃ (auxtr : auxtrace LM) mtr, exaux_traces_match extr auxtr ∧
-                               upto_stutter ls_under Ul auxtr mtr.
-Proof.
-  intros Hfb Hlr Hwp.
-  destruct (simulation_adequacy_traces
-              Σ _ _ FR e1 s1 extr Hvex Hexfirst Hfb Hlr Hwp) as [auxtr Hmatch].
-  assert (auxtrace_valid auxtr) as Hstutter.
-  { by eapply exaux_preserves_validity in Hmatch. }
-  destruct (can_destutter_auxtr auxtr) as [mtr Hupto] =>//.
-  eauto.
-Qed.
-
-Theorem simulation_adequacy_terminate Σ `{LM:LiveModel heap_lang Mdl}
-        `{!heapGpreS Σ LM} (s: stuckness)
-        e1 (s1: Mdl) FR
-        (extr : heap_lang_extrace)
-        (Hexfirst : (trfirst extr).1 = [e1])
-  :
-  (∀ mtr : @mtrace Mdl, mtrace_fairly_terminating mtr) ->
-  (* The model has finite branching *)
-  rel_finitary (sim_rel LM) →
-  live_roles Mdl s1 ≠ ∅ ->
-  (∀ `{!heapGS Σ LM},
-      ⊢ |={⊤}=>
-        frag_model_is s1 -∗
-         frag_free_roles_are (FR ∖ live_roles _ s1) -∗
-         has_fuels (Σ := Σ) 0%nat (gset_to_gmap (LM.(lm_fl) s1) (Mdl.(live_roles) s1))
-        ={⊤}=∗ WP e1 @ s; 0%nat; ⊤ {{ v, 0%nat ↦M ∅ }}
-  ) ->
-  (* The coinductive pure coq proposition given by adequacy *)
-  extrace_fairly_terminating extr.
-Proof.
-  intros Hterm Hfb Hlr Hwp Hvex Hfair.
-  destruct (simulation_adequacy_model_trace
-              Σ _ _ FR e1 s1 extr Hvex Hexfirst Hfb Hlr Hwp) as (auxtr&mtr&Hmatch&Hupto).
-  destruct (infinite_or_finite extr) as [Hinf|] =>//.
-  have Hfairaux := fairness_preserved extr auxtr Hinf Hmatch Hfair.
-  have Hvalaux := exaux_preserves_validity extr auxtr Hmatch.
-  have Hfairm := upto_stutter_fairness auxtr mtr Hupto Hfairaux.
-  have Hmtrvalid := upto_preserves_validity auxtr mtr Hupto Hvalaux.
-  have Htermtr := Hterm mtr Hmtrvalid Hfairm.
-  eapply exaux_preserves_termination =>//.
-  eapply upto_stutter_finiteness =>//.
-Qed.
-
-Theorem simulation_adequacy_terminate_ftm Σ `{FairTerminatingModel M}
-        `(LM : LiveModel heap_lang M)
-        `{!heapGpreS Σ LM} (s: stuckness)
-        e1 (s1: M) FR
-        (extr : heap_lang_extrace)
-        (Hexfirst : (trfirst extr).1 = [e1])
-  :
-  (* The model has finite branching *)
-  rel_finitary (sim_rel LM) →
-  live_roles M s1 ≠ ∅ ->
-  (∀ `{!heapGS Σ LM},
-      ⊢ |={⊤}=>
-        frag_model_is s1 -∗
-        frag_free_roles_are (FR ∖ live_roles _ s1) -∗
-        has_fuels (Σ := Σ) 0%nat (gset_to_gmap (LM.(lm_fl) s1) (M.(live_roles) s1))
-        ={⊤}=∗ WP e1 @ s; 0%nat; ⊤ {{ v, 0%nat ↦M ∅ }}
-  ) ->
-  (* The coinductive pure coq proposition given by adequacy *)
-  extrace_fairly_terminating extr.
-Proof.
-  eapply simulation_adequacy_terminate =>//.
-  apply fair_terminating_traces_terminate.
-Qed.
-
-End adequacy.
 
 (** Override the notations so that scopes and coercions work out *)
 Notation "l ↦{ q } v" := (mapsto (L:=loc) (V:=val) l (DfracOwn q) v%V)
@@ -687,11 +216,6 @@ Lemma own_proper `{inG Σ X} γ (x y: X):
   own γ x -∗ own γ y.
 Proof. by intros ->. Qed.
 
-Lemma auth_fuel_is_proper `{heapGS Σ Mdl} (x y : gmap (fmrole Mdl) nat):
-  x = y ->
-  auth_fuel_is x -∗ auth_fuel_is y.
-Proof. by intros ->. Qed.
-
 Section lifting.
 Context `{LM:LiveModel heap_lang M}.
 Context `{!heapGS Σ LM}.
@@ -703,8 +227,244 @@ Implicit Types v : val.
 Implicit Types l : loc.
 Implicit Types tid : nat.
 
+(* WIP solution for generic fuel-handling *)
+Definition sswp (s : stuckness) E e1 (Φ : expr → iProp Σ) : iProp Σ :=
+  match to_val e1 with
+  | Some v => |={E}=> (Φ (of_val v))
+  | None => ∀ σ1,
+      gen_heap_interp σ1.(heap) ={E,∅}=∗
+       ⌜if s is NotStuck then reducible e1 σ1 else True⌝ ∗
+       ∀ e2 σ2 efs,
+         ⌜prim_step e1 σ1 e2 σ2 efs⌝ ={∅}▷=∗ |={∅,E}=>
+         gen_heap_interp σ2.(heap) ∗ Φ e2 ∗ ⌜efs = []⌝
+  end%I.
 
-Lemma wp_lift_pure_step_no_fork tid E E' Φ e1 e2 fs ϕ:
+Lemma sswp_wand s e E (Φ Ψ : expr → iProp Σ) :
+  (∀ e, Φ e -∗ Ψ e) -∗ sswp s E e Φ -∗ sswp s E e Ψ.
+Proof.
+  iIntros "HΦΨ HΦ".
+  rewrite /sswp.
+  destruct (to_val e).
+  { iMod "HΦ". by iApply "HΦΨ". }
+  iIntros (?) "H".
+  iMod ("HΦ" with "H") as "[%Hs HΦ]".
+  iModIntro. iSplit; [done|].
+  iIntros (????).
+  iDestruct ("HΦ" with "[//]") as "HΦ".
+  iMod "HΦ". iIntros "!>!>". iMod "HΦ". iIntros "!>". iMod "HΦ" as "(?&?&?)".
+  iIntros "!>". iFrame.
+  by iApply "HΦΨ".
+Qed.
+
+Lemma has_fuels_decr E tid fs :
+  has_fuels_S tid fs -∗ |~{E}~| has_fuels tid fs.
+Proof.
+  iIntros "Hf".
+  rewrite weakestpre.pre_step_unseal.
+  iIntros (extr atr) "[%Hvse [Hσ Hm]]".
+  iMod (model_state_interp_has_fuels_decr with "Hm Hf") as "[Hm Hf]".
+  by iFrame.
+Qed.
+
+Lemma has_fuels_dealloc E tid fs ρ δ :
+  ρ ∉ live_roles _ δ →
+  frag_model_is δ -∗
+  has_fuels tid fs -∗
+  |~{E}~| frag_model_is δ ∗ has_fuels tid (delete ρ fs).
+Proof.
+  iIntros (Hnin) "Hst Hf".
+  rewrite weakestpre.pre_step_unseal.
+  iIntros (extr atr) "[%Hvse [Hσ Hm]]".
+  iMod (model_state_interp_has_fuels_dealloc with "Hm Hst Hf") as "[Hm Hf]";
+    [done|].
+  by iFrame.
+Qed.
+
+(* Sanity check: Rule from paper *)
+Lemma wp_role_dealloc s tid E e fs ρ δ Φ :
+  ρ ∉ live_roles _ δ →
+  frag_model_is δ -∗
+  has_fuels tid fs -∗
+  (frag_model_is δ -∗ has_fuels tid (delete ρ fs) -∗ WP e @ s; tid; E {{ Φ }}) -∗
+  WP e @ s; tid; E {{ Φ }}.
+Proof.
+  iIntros (Hnin) "HM Hfuels Hwp".
+  (* TODO: add typeclass to allow iMod'ing pre_step mods under WP's *)
+  iApply pre_step_wp.
+  iMod (has_fuels_dealloc with "HM Hfuels") as "[HM Hfuels]"; [done|].
+  iIntros "!>". by iApply ("Hwp" with "HM Hfuels").
+Qed.
+
+Lemma wp_step_model s tid ρ (f1 : nat) fs fr s1 s2 E e Φ :
+  TCEq (to_val e) None →
+  M.(live_roles) s2 ⊆ M.(live_roles) s1 →
+  ρ ∉ dom fs →
+  fmtrans M s1 (Some ρ) s2 →
+  ▷ frag_model_is s1 -∗ ▷ has_fuels tid ({[ρ:=f1]} ∪ fmap S fs) -∗
+  ▷ frag_free_roles_are fr -∗
+  sswp s E e (λ e', frag_model_is s2 -∗ frag_free_roles_are fr -∗
+                    has_fuels tid ({[ρ:=(LM.(lm_fl) s2)]} ∪ fs) -∗
+                    WP e' @ s; tid; E {{ Φ }} ) -∗
+  WP e @ s; tid; E {{ Φ }}.
+Proof.
+  iIntros (Hval Hlive Hdom Htrans) ">Hst >Hfuel1 >Hfr Hwp".
+  rewrite wp_unfold /wp_pre.
+  rewrite /sswp. simpl. rewrite Hval.
+  iIntros (extr atr K tp1 tp2 σ1 Hvalid Hloc Hexend) "(% & Hsi & Hmi)".
+  iMod ("Hwp" with "Hsi") as (Hred) "Hwp".
+  iIntros "!>".
+  iSplitR; [by rewrite Hexend in Hred|].
+  iIntros (????).
+  rewrite Hexend.
+  iMod ("Hwp" with "[//]") as "Hwp". iIntros "!>!>". iMod "Hwp". iIntros "!>".
+  iApply step_fupdN_intro; [done|]. iIntros "!>".
+  iMod "Hwp" as "[Hσ [Hwp ->]]".
+  iDestruct (model_agree' with "Hmi Hst") as %Hmeq.
+  iFrame.
+  rewrite /trace_ends_in in Hexend.
+  rewrite -Hexend.
+  iMod (update_model_step with "Hfuel1 Hst Hmi") as
+    (δ2 Hvse) "(Hfuel & Hst & Hmod)"; eauto.
+  - rewrite -Hloc.
+    eapply locale_step_atomic; eauto.
+    by apply fill_step.
+  - iModIntro; iExists δ2, (Take_step ρ tid).
+    rewrite big_sepL_nil. iFrame.
+    iSplit.
+    { iPureIntro. simpl in *. naive_solver. }
+    iDestruct ("Hwp" with "Hst Hfr Hfuel") as "Hwp". by iFrame.
+Qed.
+
+Lemma wp_step_model_singlerole s tid ρ (f1 : nat) fr s1 s2 E e Φ :
+  TCEq (to_val e) None →
+  M.(live_roles) s2 ⊆ M.(live_roles) s1 →
+  fmtrans M s1 (Some ρ) s2 →
+  ▷ frag_model_is s1 -∗ ▷ has_fuel tid ρ f1 -∗ ▷ frag_free_roles_are fr -∗
+  sswp s E e (λ e', frag_model_is s2 -∗ frag_free_roles_are fr -∗
+                    has_fuel tid ρ (LM.(lm_fl) s2) -∗
+                    WP e' @ s; tid; E {{ Φ }} ) -∗
+  WP e @ s; tid; E {{ Φ }}.
+Proof.
+  iIntros (Hval Hlive Htrans) ">Hst >Hfuel1 >Hfr Hwp".
+  rewrite has_fuel_fuels.
+  replace ({[ρ := f1]}) with ({[ρ := f1]} ∪ (fmap S ∅:gmap _ _)); last first.
+  { rewrite fmap_empty. rewrite right_id_L. done. }
+  iApply (wp_step_model with "Hst Hfuel1 Hfr"); [done|set_solver|done|].
+  (* This can be done with Proper instances of sswp too *)
+  iApply (sswp_wand with "[] Hwp").
+  iIntros (e') "Hwp Hst Hfuel1 Hfr".
+  rewrite has_fuel_fuels. rewrite right_id_L.
+  iApply ("Hwp" with "Hst Hfuel1 Hfr").
+Qed.
+
+Lemma wp_step_fuel s tid E e fs Φ :
+  fs ≠ ∅ →
+  has_fuels_S tid fs -∗
+  sswp s E e (λ e', has_fuels tid fs -∗ WP e' @ s; tid; E {{ Φ }} ) -∗
+  WP e @ s; tid; E {{ Φ }}.
+Proof.
+  iIntros (?) "HfuelS Hwp".
+  rewrite wp_unfold /wp_pre /sswp /=.
+  destruct (to_val e).
+  { (* This should be possible without fupd_pre_step? Probably import stuff. *)
+    iMod (has_fuels_decr with "HfuelS") as "Hfuel".
+    iDestruct ("Hwp" with "Hfuel") as "Hwp".
+    iDestruct (wp_value_inv with "Hwp") as "Hwp".
+    iApply fupd_pre_step. iMod "Hwp". by iIntros "!>!>". }
+  iIntros (extr atr K tp1 tp2 σ1 Hvalid Hloc Hends) "(%Hvalid' & Hsi & Hmi)".
+  rewrite Hends.
+  iMod ("Hwp" with "Hsi") as (Hred) "Hwp".
+  iModIntro. iSplit; [done|].
+  iIntros (e2 σ2 efs Hstep).
+  iMod ("Hwp" with "[//]") as "Hwp".
+  iIntros "!>!>". iMod "Hwp". iIntros "!>".
+  iApply step_fupdN_intro; [done|]. iIntros "!>".
+  iMod "Hwp".
+  rewrite -Hends.
+  iMod (update_fuel_step with "HfuelS Hmi") as (δ2) "(%Hvse & Hfuel & Hmod)" =>//.
+  { rewrite Hends -Hloc. eapply locale_step_atomic; eauto. by apply fill_step. }
+  iIntros "!>".
+  iDestruct "Hwp" as "[Hsi [Hwp ->]]".
+  iExists _, (Silent_step tid). iFrame. iSplit; [done|].
+  iDestruct ("Hwp" with "Hfuel") as "Hwp". iSplit; [|done].
+  iApply (wp_wand with "Hwp").
+  iIntros (v) "HΦ'". iFrame.
+Qed.
+
+(** Fork: Not using Texan triples to avoid some unnecessary [True] *)
+Lemma wp_role_fork s tid E e Φ R1 R2 (Hdisj: R1 ##ₘ R2) (Hnemp: R1 ∪ R2 ≠ ∅):
+  has_fuels_S tid (R1 ∪ R2) -∗
+  (∀ tid', ▷ (has_fuels tid' R2 -∗ WP e @ s; tid'; ⊤ {{ _, tid' ↦M ∅ }})) -∗
+  ▷ (has_fuels tid R1 ={E}=∗ Φ (LitV LitUnit)) -∗
+  WP Fork e @ s; tid; E {{ Φ }}.
+Proof.
+  iIntros "Htid He HΦ". iApply wp_lift_atomic_head_step; [done|].
+  iIntros (extr auxtr K tp1 tp2 σ1 Hvalex Hexend Hloc) "(% & Hsi & Hmi)".
+  iMod (update_fork_step R1 R2 _
+       (tp1 ++ ectx_language.fill K (Val $ LitV LitUnit) :: tp2 ++ [e])
+       _ _ _ e _ σ1 with "Htid Hmi") as
+    (δ2 Hvse) "(Hfuels1 & Hfuels2 & Hmi)".
+  { done. }
+  { done. }
+  { rewrite /trace_ends_in in Hexend. rewrite Hexend. done. }
+  { rewrite -Hloc. rewrite -(language.locale_fill _ _ K).
+    rewrite /trace_ends_in in Hexend. rewrite Hexend.
+    econstructor 1 =>//.
+    apply fill_step, head_prim_step. econstructor. }
+  { list_simplifier. exists (tp1 ++ fill K #() :: tp2).
+    rewrite /trace_ends_in in Hexend. rewrite Hexend.
+    split; first by list_simplifier. simpl.
+    admit. }
+    (* rewrite app_length //=. } *)
+  iModIntro. iSplit. iPureIntro; first by eauto. iNext.
+  iIntros (e2 σ2 efs Hstep).
+  have [-> [-> ->]] : σ2 = σ1 ∧ efs = [e] ∧ e2 = Val $ LitV LitUnit by inv_head_step.
+  iMod ("HΦ" with "Hfuels1") as "HΦ". iModIntro. iExists δ2, (Silent_step tid).
+  iFrame.
+  rewrite Hexend /=. iFrame "Hsi".
+  iSplit; first by iPureIntro.
+  iSplit; [|done].
+  iApply "He". by list_simplifier.
+Admitted.
+
+Lemma sswp_pure_step s E e1 e2 (Φ : Prop) Ψ :
+  PureExec Φ 1 e1 e2 → Φ → Ψ e2 -∗ sswp s E e1 Ψ%I.
+Proof.
+  iIntros (Hpe HΦ) "HΨ".
+  assert (pure_step e1 e2) as Hps.
+  { specialize (Hpe HΦ). by apply nsteps_once_inv in Hpe. }
+  rewrite /sswp /=.
+  assert (to_val e1 = None) as ->.
+  { destruct Hps as [Hred _].
+    specialize (Hred (Build_state ∅ ∅)).
+    by eapply reducible_not_val. }
+  iIntros (σ) "Hσ".
+  iMod fupd_mask_subseteq as "Hclose"; last iModIntro; first by set_solver.
+  iSplit.
+  { destruct s; [|done]. by destruct Hps as [Hred _]. }
+  iIntros (e2' σ2 efs Hstep) "!>!>!>".
+  iMod "Hclose". iModIntro.
+  destruct Hps as [_ Hstep'].
+  apply Hstep' in Hstep as [-> [-> ->]].
+  iFrame. done.
+Qed.
+
+(* Sanity check *)
+Lemma wp_lift_pure_step_no_fork_alt tid E Φ e1 e2 fs ϕ :
+  fs ≠ ∅ ->
+  PureExec ϕ 1 e1 e2 ->
+  ϕ ->
+  has_fuels_S tid fs -∗
+  (has_fuels tid fs -∗ WP e2 @ tid; E {{ Φ }}) -∗
+  WP e1 @ tid; E {{ Φ }}.
+Proof.
+  intros NnO Hpe Hϕ.
+  iIntros "Hfuel Hwp".
+  iApply (wp_step_fuel with "Hfuel"); [done|].
+  by iApply sswp_pure_step.
+Qed.
+
+Lemma wp_lift_pure_step_no_fork tid E E' Φ e1 e2 fs ϕ :
   fs ≠ ∅ ->
   PureExec ϕ 1 e1 e2 ->
   ϕ ->
@@ -724,198 +484,15 @@ Proof.
   simplify_eq. iMod "Hclose" as "_". iMod "H" as "[Hfuels Hkont]".
   rewrite !app_nil_r.
   iDestruct "Hsi" as "(%&Hgh&Hmi)".
-  (* iDestruct "Hmi" as (??) "(?&?&?&?&?&?&%)". *)
-
-  iMod (update_no_step_enough_fuel _ _ ∅ with "Hfuels Hmi") as "H"; eauto;
-    [by intros X%dom_empty_inv_L | set_solver | set_solver | econstructor =>//; by apply fill_step |].
+  iMod (update_fuel_step with "Hfuels Hmi") as "H";
+    [done | econstructor =>//; by apply fill_step | ].
   iModIntro.
-  iDestruct ("H") as (δ2 ℓ [Hlabels Hvse]) "[Hfuels Hmi]".
-  iExists δ2, ℓ.
+  iDestruct ("H") as (δ2 Hvse) "[Hfuels Hmi]".
+  iExists δ2, (Silent_step $ (language.locale_of tp1 (ectx_fill K e1))).
   rewrite /state_interp /=.
   rewrite Hexend /=. list_simplifier. iFrame "Hgh Hmi".
-  repeat iSplit; last done.
-  - iPureIntro. destruct ℓ =>//.
-  - iPureIntro. destruct Hvse as (?&?&? )=>//.
-  - iPureIntro. destruct Hvse as (?&?&? )=>//.
-  - iApply "Hkont". iApply (has_fuels_proper with "Hfuels") =>//.
-    rewrite map_filter_id //. intros ?? ?%elem_of_dom_2; set_solver.
-Qed.
-
-Lemma wp_lift_pure_step_no_fork_remove_role rem s tid E E' Φ e1 e2 fs ϕ:
-  fs ≠ ∅ ->
-  rem ⊆ dom fs →
-  rem ∩ live_roles _ s = ∅ →
-  PureExec ϕ 1 e1 e2 ->
-  ϕ ->
-  (|={E}[E']▷=> frag_model_is s ∗ has_fuels_S tid fs ∗
-                 (frag_model_is s -∗ (has_fuels tid (fs ⇂ (dom fs ∖ rem))) -∗ WP e2 @ tid; E {{ Φ }}))
-  ⊢ WP e1 @ tid; E {{ Φ }}.
-Proof.
-  intros NnO Hincl Hdisj Hpe Hϕ.
-  have Hps: pure_step e1 e2.
-  { specialize (Hpe Hϕ). by apply nsteps_once_inv in Hpe. }
-  iIntros "H". iApply wp_lift_step; eauto.
-  { destruct Hps as [Hred _]. specialize (Hred inhabitant). eapply reducible_not_val; eauto. }
-  iIntros (extr auxtr K tp1 tp2 σ1 Hvalex Hexend Hloc) "Hsi".
-  iMod "H". iMod fupd_mask_subseteq as "Hclose"; last iModIntro; first by set_solver.
-  iSplit; first by destruct Hps as [Hred _].
-  iNext. iIntros (e2' σ2 efs Hpstep).
-  destruct Hps as [? Hdet]. specialize (Hdet _ _ _ _ Hpstep) as (?&?&?).
-  simplify_eq. iMod "Hclose" as "_". iMod "H" as "(Hmod & Hfuels & Hkont)".
-  rewrite !app_nil_r.
-  iDestruct "Hsi" as "(%&Hgh&Hmi)".
-  iDestruct (model_agree' with "Hmi Hmod") as %Heq.
-
-  iMod (update_no_step_enough_fuel _ _ rem with "Hfuels Hmi") as "H"; eauto;
-    [by intros X%dom_empty_inv_L | set_solver | econstructor =>//; by apply fill_step |].
-  iModIntro.
-  iDestruct ("H") as (δ2 ℓ [Hlabels Hvse]) "[Hfuels Hmi]".
-  iExists δ2, ℓ.
-  rewrite /state_interp /=.
-  rewrite Hexend /=. list_simplifier. iFrame "Hgh Hmi".
-  repeat iSplit; last done.
-  - iPureIntro. destruct ℓ =>//.
-  - iPureIntro. destruct Hvse as (?&?&? )=>//.
-  - iPureIntro. destruct Hvse as (?&?&? )=>//.
-  - iApply ("Hkont" with "Hmod"). iApply (has_fuels_proper with "Hfuels") =>//.
-Qed.
-
-(* Lemma wp_lift_pure_step_no_fork_2 tid E E' Φ e1 e2 (fs: gmap (fmrole Mdl) nat) R ϕ: *)
-(*   R ≠ ∅ -> *)
-(*   PureExec ϕ 1 e1 e2 -> *)
-(*   ϕ -> *)
-(*   (forall (ρ: fmrole Mdl) (f: nat), fs !! ρ = Some f -> f > 0) -> *)
-(*   (|={E}[E']▷=> has_fuels tid R fs ∗ ((has_fuels tid R (fmap (λ (x: nat), (x - 1)%nat) fs)) -∗ WP e2 @ tid; E {{ Φ }})) *)
-(*   ⊢ WP e1 @ tid; E {{ Φ }}. *)
-(* Proof. *)
-
-Lemma wp_lift_pure_step_no_fork' fs tid E E' Φ e1 e2:
-  fs ≠ ∅ ->
-  PureExec True 1 e1 e2 ->
-  (|={E}[E']▷=> has_fuels_S tid fs ∗ ((has_fuels tid fs) -∗ WP e2 @ tid; E {{ Φ }}))
-  ⊢ WP e1 @ tid; E {{ Φ }}.
-Proof.
-  intros. by iApply wp_lift_pure_step_no_fork.
-Qed.
-
-Lemma wp_lift_pure_step_no_fork_singlerole tid E E' Φ e1 e2 ρ f φ:
-  PureExec φ 1 e1 e2 -> φ ->
-  (|={E}[E']▷=> has_fuel tid ρ (S f) ∗ ((has_fuel tid ρ f) -∗ WP e2 @ tid; E {{ Φ }}))
-  ⊢ WP e1 @ tid; E {{ Φ }}.
-Proof.
-  iIntros (??) "H". rewrite has_fuel_fuels_S.
-  iApply (wp_lift_pure_step_no_fork {[ ρ := f ]} {[ρ]}); eauto; last first.
-  rewrite has_fuel_fuels //. apply map_non_empty_singleton.
-Qed.
-
-Lemma wp_lift_pure_step_no_fork_take_step s1 s2 tid E E' fs1 fs2 fr1 Φ e1 e2 ρ φ:
-  PureExec φ 1 e1 e2 -> φ ->
-  valid_new_fuelmap (LM := LM) fs1 fs2 s1 s2 ρ ->
-  live_roles M s2 ∖ live_roles M s1 ⊆ fr1 →
-  M.(fmtrans) s1 (Some ρ) s2 ->
-  (|={E}[E']▷=> frag_model_is s1 ∗ has_fuels tid fs1 ∗ frag_free_roles_are fr1 ∗
-                 (frag_model_is s2 -∗ frag_free_roles_are (fr1 ∖ (live_roles M s2 ∖ live_roles M s1))
-                  -∗ (has_fuels tid fs2 -∗ WP e2 @ tid; E {{ Φ }})))
-  ⊢ WP e1 @ tid; E {{ Φ }}.
-Proof.
-  iIntros (Hpe Hφ Hval Hfr Htrans).
-  have Hps: pure_step e1 e2.
-  { specialize (Hpe Hφ). by apply nsteps_once_inv in Hpe. }
-  iIntros "Hkont".
-  iApply wp_lift_step; eauto.
-  { destruct (pure_step_safe _ e2 Hps inhabitant) as (?&?&?&?). by eapply val_stuck. }
-
-  iIntros (extr auxtr K tp1 tp2 σ1 Hvalex Hexend Hloc) "Hsi".
-  iMod "Hkont". iMod fupd_mask_subseteq as "Hclose"; last iModIntro; first by set_solver.
-  iSplit; first by destruct Hps as [Hred _].
-  iNext. iIntros (e2' σ2 efs Hpstep).
-  destruct Hps as [? Hdet]. specialize (Hdet _ _ _ _ Hpstep) as (?&?&?).
-  simplify_eq. iMod "Hclose" as "_". iMod "Hkont" as "(Hmod&Hfuels&Hfr&Hkont)".
-  rewrite !app_nil_r.
-  iDestruct "Hsi" as "(%&Hgh&Hmi)". simpl.
-  iDestruct (model_agree' with "Hmi Hmod") as %Hmeq.
-
-  iMod (update_step_still_alive _ _ _ _ σ1 σ1 with "Hfuels Hmod Hmi Hfr") as "H"; eauto.
-  { rewrite Hexend. eauto. }
-  { econstructor =>//.
-    - rewrite Hexend //=.
-    - by apply fill_step. }
-  { rewrite Hmeq. apply Hval. }
-  iModIntro. iDestruct "H" as (δ2 ℓ [Hlabels Hvse]) "(Hfuels&Hmod&Hmi&Hfr)".
-  iExists δ2, ℓ.
-  rewrite Hexend /=. list_simplifier. iFrame "Hgh Hmi".
-  repeat iSplit; last done.
-  - iPureIntro. destruct ℓ =>//.
-  - iPureIntro. destruct Hvse as (?&?&? )=>//.
-  - iPureIntro. destruct Hvse as (?&?&? )=>//.
-  - by iSpecialize ("Hkont" with "Hmod Hfr Hfuels").
-Qed.
-
-Lemma wp_lift_pure_step_no_fork_singlerole_take_step s1 s2 tid E E' (f1 f2: nat) fr Φ e1 e2 ρ φ:
-  PureExec φ 1 e1 e2 -> φ ->
-  live_roles _ s2 ⊆ live_roles _ s1 ->
-  (f2 ≤ LM.(lm_fl) s2)%nat -> M.(fmtrans) s1 (Some ρ) s2 ->
-  (|={E}[E']▷=> frag_model_is s1 ∗ frag_free_roles_are fr ∗ has_fuel tid ρ f1 ∗
-   (frag_model_is s2 -∗ frag_free_roles_are fr -∗ (if decide (ρ ∈ live_roles M s2) then has_fuel tid ρ f2 else tid ↦M ∅) -∗
-                               WP e2 @ tid; E {{ Φ }}))
-  ⊢ WP e1 @ tid; E {{ Φ }}.
-Proof.
-  iIntros (Hpe Hφ Hroles Hfl Hmdl).
-  rewrite has_fuel_fuels.
-  iIntros "H".
-  iApply (wp_lift_pure_step_no_fork_take_step _ _ _ _ _ {[ρ := f1]}
-         (if decide (ρ ∈ live_roles M s2) then {[ρ := f2]} else ∅) fr  with "[H]"); eauto.
-  - repeat split.
-    + intros ?. rewrite decide_True //. rewrite lookup_singleton //=.
-    + destruct (decide (ρ ∈ live_roles _ s2)); set_solver.
-    + set_solver.
-    + intros ρ' Hdom. destruct (decide (ρ ∈ live_roles M s2)); set_solver.
-    + intros ρ' Hneq Hin. destruct (decide (ρ ∈ live_roles M s2)); set_solver.
-    + destruct (decide (ρ ∈ live_roles M s2)); set_solver.
-    + destruct (decide (ρ ∈ live_roles M s2)); set_solver.
-  - set_solver.
-  - iMod "H". do 2 iModIntro. iMod "H" as "(Hmod&Hfr&Hfuels&Hkont)". iModIntro.
-    iFrame "Hmod Hfr Hfuels". iIntros "Hmod Hfr Hfuels". iApply ("Hkont" with "Hmod [Hfr] [Hfuels]").
-    + replace (fr ∖ (live_roles M s2 ∖ live_roles M s1)) with fr; [done|set_solver].
-    + destruct (decide (ρ ∈ live_roles M s2)).
-      * rewrite -has_fuel_fuels //.
-      * iDestruct "Hfuels" as "[Hf _]". rewrite dom_empty_L //.
-Qed.
-
-Lemma wp_lift_pure_step_no_fork_singlerole' tid E E' Φ e1 e2 ρ f:
-  PureExec True 1 e1 e2 ->
-  (|={E}[E']▷=> has_fuel tid ρ (S f) ∗ ((has_fuel tid ρ f) -∗ WP e2 @ tid; E {{ Φ }}))
-  ⊢ WP e1 @ tid; E {{ Φ }}.
-Proof.
-  iIntros (?) "H". rewrite has_fuel_fuels_S.
-  iApply (wp_lift_pure_step_no_fork' {[ ρ := f ]} {[ρ]}); last first.
-  rewrite has_fuel_fuels //. apply map_non_empty_singleton.
-Qed.
-
-(** Fork: Not using Texan triples to avoid some unnecessary [True] *)
-Lemma wp_fork_nostep s tid E e Φ R1 R2 fs (Hdisj: R1 ## R2) (Hnemp: fs ≠ ∅):
-  R1 ∪ R2 = dom fs ->
-  (∀ tid', ▷ (has_fuels tid' (fs ⇂ R2) -∗ WP e @ s; tid'; ⊤ {{ _, tid' ↦M ∅ }})) -∗
-     ▷ (has_fuels tid (fs ⇂ R1) ={E}=∗ Φ (LitV LitUnit)) -∗
-     has_fuels_S tid fs -∗ WP Fork e @ s; tid; E {{ Φ }}.
-Proof.
-  iIntros (Hunioneq) "He HΦ Htid". iApply wp_lift_atomic_head_step; [done|].
-  iIntros (extr auxtr K tp1 tp2 σ1 Hvalex Hexend Hloc) "(% & Hsi & Hmi)".
-  iMod (update_fork_split R1 R2 _
-       (tp1 ++ ectx_language.fill K (Val $ LitV LitUnit) :: tp2 ++ [e]) fs _ _ _ e _ σ1 with "Htid Hmi") as
-       (δ2) "(Hfuels2 & Hfuels1 & Hσ & %Hvse)" => //.
-  { rewrite -Hloc. rewrite -(language.locale_fill _ _ K). econstructor 1 =>//.
-    apply fill_step, head_prim_step. econstructor. }
-  { list_simplifier. exists (tp1 ++ fill K #() :: tp2). split; first by list_simplifier.
-    rewrite !app_length //=. }
-  iModIntro. iSplit. iPureIntro; first by eauto. iNext.
-  iIntros (e2 σ2 efs Hstep).
-  have [-> [-> ->]] : σ2 = σ1 ∧ efs = [e] ∧ e2 = Val $ LitV LitUnit by inv_head_step.
-  iMod ("HΦ" with "Hfuels1") as "HΦ". iModIntro. iExists δ2, (Silent_step tid). iFrame.
-  rewrite Hexend /=. iFrame "Hsi".
-  iSplit; first by iPureIntro.
-  iSplit; [|done].
-  iApply "He". by list_simplifier.
+  repeat iSplit; try naive_solver.
+  iApply "Hkont". iApply (has_fuels_proper with "Hfuels") =>//.
 Qed.
 
 (** Heap *)
@@ -953,134 +530,131 @@ Proof.
   rewrite big_opM_singleton; iDestruct "Hvs" as "[$ Hvs]". by iApply "IH".
 Qed.
 
-(* TODO *)
-
-Lemma wp_allocN_seq_nostep s tid E v n fs:
-  fs ≠ ∅ ->
+Lemma sswp_allocN_seq s tid E v n (Φ : expr → iProp Σ) :
   0 < n →
-  {{{ has_fuels_S tid fs }}} AllocN (Val $ LitV $ LitInt $ n) (Val v) @ s; tid; E
-  {{{ l, RET LitV (LitLoc l); has_fuels tid fs ∗ [∗ list] i ∈ seq 0 (Z.to_nat n),
-      (l +ₗ (i : nat)) ↦ v ∗ meta_token (l +ₗ (i : nat)) ⊤ }}}.
+  ▷ (∀ (l:loc), ([∗ list] i ∈ seq 0 (Z.to_nat n),
+                 (l +ₗ (i : nat)) ↦ v ∗ meta_token (l +ₗ (i : nat)) ⊤) -∗ Φ #l) -∗
+  sswp s E (AllocN (Val $ LitV $ LitInt $ n) (Val v)) Φ.
 Proof.
-  iIntros (HnO Hn Φ) "HfuelS HΦ". iApply wp_lift_atomic_head_step_no_fork; auto.
-  iIntros (extr auxtr K tp1 tp2 σ1 Hvalex Hexend Hloc) "(% & Hsi & Hmi)".
-  iModIntro; iSplit; first by eauto.
-  iIntros (e2 σ2 efs Hstep). iNext.
+  iIntros (HnO) "HΦ".
+  rewrite /sswp. simpl.
+  iIntros (σ) "Hσ".
+  iMod fupd_mask_subseteq as "Hclose"; last iModIntro; first by set_solver.
+  iSplit.
+  { iPureIntro. destruct s; [|done]. apply head_prim_reducible. eauto. }
+  iIntros (e2 σ2 efs Hstep). iIntros "!>!>!>".
+  iMod "Hclose".
+  apply head_reducible_prim_step in Hstep; [|eauto].
   inv_head_step.
-  iMod (gen_heap_alloc_big _ (heap_array l (replicate (Z.to_nat n) v)) with "Hsi")
-    as "(Hsi & Hl & Hm)".
+  iMod (gen_heap_alloc_big _ (heap_array l (replicate (Z.to_nat n) v)) with "Hσ")
+    as "(Hσ & Hl & Hm)".
   { apply heap_array_map_disjoint.
     rewrite replicate_length Z2Nat.id ?Hexend; auto with lia. }
-  iMod (update_no_step_enough_fuel _ _ ∅ with "HfuelS Hmi") as (δ2 ℓ) "([%Hlabel %Hvse] & Hfuel & Hmi)" =>//.
-  { by intros ?%dom_empty_inv_L. }
-  { set_solver. }
-  { rewrite Hexend. apply head_locale_step. by econstructor. }
-  iModIntro; iExists δ2, ℓ.
-  rewrite Hexend //=. iFrame "Hmi Hsi".
-  repeat iSplit =>//.
-  iApply "HΦ". iSplitL "Hfuel".
-  { iApply (has_fuels_proper with "Hfuel") =>//.
-    rewrite map_filter_id //. intros ???%elem_of_dom_2; set_solver. }
+  iFrame.
+  iModIntro.
+  iSplit; [|done].
+  iApply "HΦ".
   iApply big_sepL_sep. iSplitL "Hl".
   + by iApply heap_array_to_seq_mapsto.
   + iApply (heap_array_to_seq_meta with "Hm"). by rewrite replicate_length.
 Qed.
 
-Lemma wp_alloc_nostep s tid E v fs :
-  fs ≠ ∅ ->
-  {{{ has_fuels_S tid fs }}} Alloc (Val v) @ s; tid; E {{{ l, RET LitV (LitLoc l); l ↦ v ∗ meta_token l ⊤ ∗ has_fuels tid fs }}}.
+Lemma wp_choose_nat s E (Φ : expr → iProp Σ) :
+  (∀ (n:nat), Φ $ Val $ LitV (LitInt n)) -∗
+  sswp s E ChooseNat Φ.
 Proof.
-  iIntros (? Φ) "HfuelS HΦ". iApply (wp_allocN_seq_nostep with "HfuelS"); auto with lia.
-  iIntros "!>" (l) "/= (? & ? & _)". rewrite loc_add_0. by iApply "HΦ"; iFrame.
-Qed.
-
-Lemma wp_choose_nat_nostep s tid E fs :
-  fs ≠ ∅ ->
-  {{{ has_fuels_S tid fs }}}
-    ChooseNat @ s; tid; E
-  {{{ (n:nat), RET LitV (LitInt n); has_fuels tid fs }}}.
-Proof.
-  iIntros (? Φ) "HfuelS HΦ". iApply wp_lift_atomic_head_step_no_fork; auto.
-  iIntros (extr auxtr K tp1 tp2 σ1 Hvalex Hexend Hloc) "(% & Hsi & Hmi)".
-  iModIntro; iSplit; eauto.
-  (* TODO: Improve this so we hide the (arbitrary) choice of `n` *)
-  Unshelve. 2: apply O.
-  iIntros (e2 σ2 efs Hstep). iNext.
+  iIntros "HΦ".
+  rewrite /sswp. simpl.
+  iIntros (σ) "Hσ".
+  iMod fupd_mask_subseteq as "Hclose"; last iModIntro; first by set_solver.
+  iSplit.
+  { iPureIntro. destruct s; [|done]. apply head_prim_reducible. eauto. }
+  iIntros (e2 σ2 efs Hstep). iIntros "!>!>!>".
+  iMod "Hclose".
+  apply head_reducible_prim_step in Hstep; [|eauto].
   inv_head_step.
-  iMod (update_no_step_enough_fuel _ _ ∅ with "HfuelS Hmi") as (δ2 ℓ) "([%Hlabel %Hvse] & Hfuel & Hmi)" =>//.
-  { by intros ?%dom_empty_inv_L. }
-  { set_solver. }
-  { rewrite Hexend. apply head_locale_step. by econstructor. }
-  iModIntro; iExists δ2, ℓ.
-  rewrite Hexend //=. iFrame "Hmi Hsi".
-  repeat iSplit =>//.
+  iFrame.
+  iModIntro.
+  iSplit; [|done].
   iApply "HΦ".
-  iApply (has_fuels_proper with "Hfuel") =>//.
-  rewrite map_filter_id //. intros ???%elem_of_dom_2; set_solver.
+  (* TODO: Improve this so we hide the (arbitrary) choice of `n` *)
+  Unshelve. all: apply O.
 Qed.
 
-Lemma wp_load_nostep s tid E l q v fs:
-  fs ≠ ∅ ->
-  {{{ ▷ l ↦{q} v ∗ has_fuels_S tid fs }}} Load (Val $ LitV $ LitLoc l) @ s; tid; E {{{ RET v; l ↦{q} v ∗ has_fuels tid fs }}}.
+(* Lemma wp_choose_nat_nostep s tid E fs : *)
+(*   fs ≠ ∅ -> *)
+(*   {{{ has_fuels_S tid fs }}} *)
+(*     ChooseNat @ s; tid; E *)
+(*   {{{ (n:nat), RET LitV (LitInt n); has_fuels tid fs }}}. *)
+(* Proof. *)
+(*   iIntros (? Φ) "HfuelS HΦ". iApply wp_lift_atomic_head_step_no_fork; auto. *)
+(*   iIntros (extr auxtr K tp1 tp2 σ1 Hvalex Hexend Hloc) "(% & Hsi & Hmi)". *)
+(*   iModIntro; iSplit; eauto. *)
+(*   (* TODO: Improve this so we hide the (arbitrary) choice of `n` *) *)
+(*   Unshelve. 2: apply O. *)
+(*   iIntros (e2 σ2 efs Hstep). iNext. *)
+(*   inv_head_step. *)
+(*   iMod (update_no_step_enough_fuel _ _ ∅ with "HfuelS Hmi") as (δ2 ℓ) "([%Hlabel %Hvse] & Hfuel & Hmi)" =>//. *)
+(*   { by intros ?%dom_empty_inv_L. } *)
+(*   { set_solver. } *)
+(*   { rewrite Hexend. apply head_locale_step. by econstructor. } *)
+(*   iModIntro; iExists δ2, ℓ. *)
+(*   rewrite Hexend //=. iFrame "Hmi Hsi". *)
+(*   repeat iSplit =>//. *)
+(*   iApply "HΦ". *)
+(*   iApply (has_fuels_proper with "Hfuel") =>//. *)
+(*   rewrite map_filter_id //. intros ???%elem_of_dom_2; set_solver. *)
+(* Qed. *)
+
+Lemma wp_load s E l q v (Φ : expr → iProp Σ) :
+  ▷ l ↦{q} v -∗
+  ▷ (l ↦{q} v -∗ Φ v) -∗
+  sswp s E (Load (Val $ LitV $ LitLoc l)) Φ.
 Proof.
-  iIntros (? Φ) "[>Hl HfuelS] HΦ". iApply wp_lift_atomic_head_step_no_fork; auto.
-  iIntros (extr atr K tp1 tp2 σ1 Hval Hexend Hloc) "(% & Hsi & Hmi) !>".
-  iDestruct (@gen_heap_valid with "Hsi Hl") as %Hheap.
-  iSplit; first by rewrite Hexend // in Hheap;  eauto. iIntros "!>" (e2 σ2 efs Hstep).
-  rewrite Hexend in Hheap. inv_head_step.
-  iMod (update_no_step_enough_fuel _ _ ∅ with "HfuelS Hmi") as (δ2 ℓ) "([%Hlabels %Hvse] & Hfuel & Hmod)" =>//.
-  { by intros ?%dom_empty_inv_L. }
-  { set_solver. }
-  { rewrite Hexend. apply head_locale_step. by econstructor. }
-  iModIntro; iExists _,_.
-  rewrite Hexend //=. iFrame "Hsi Hmod".
-  do 2 (iSplit=>//).
-  iApply "HΦ". iFrame. iApply (has_fuels_proper with "Hfuel") =>//.
-  rewrite map_filter_id //. intros ???%elem_of_dom_2; set_solver.
+  iIntros ">Hl HΦ".
+  rewrite /sswp. simpl.
+  iIntros (σ) "Hσ".
+  iMod fupd_mask_subseteq as "Hclose"; last iModIntro; first by set_solver.
+  iDestruct (@gen_heap_valid with "Hσ Hl") as %Hheap.
+  iSplit.
+  { iPureIntro. destruct s; [|done]. apply head_prim_reducible. eauto. }
+  iIntros (e2 σ2 efs Hstep). iIntros "!>!>!>".
+  iMod "Hclose".
+  apply head_reducible_prim_step in Hstep; [|eauto].
+  inv_head_step.
+  iFrame.
+  iModIntro.
+  iSplit; [|done].
+  by iApply "HΦ".
 Qed.
 
-Lemma wp_store_nostep s tid E l v' v fs:
-  fs ≠ ∅ ->
-  {{{ ▷ l ↦ v' ∗ has_fuels_S tid fs }}}
-    Store (Val $ LitV (LitLoc l)) (Val v) @ s; tid; E
-  {{{ RET LitV LitUnit; l ↦ v ∗ has_fuels tid fs }}}.
-Proof.
-  iIntros (? Φ) "[>Hl HfuelS] HΦ".
-  iApply wp_lift_atomic_head_step_no_fork; auto.
-  iIntros (extr atr K tp1 tp2 σ1 Hval Hexend Hloc) "(% & Hsi & Hmi) !>".
-  iDestruct (@gen_heap_valid with "Hsi Hl") as %Hheap.
-  iSplit; first by rewrite Hexend // in Hheap;  eauto. iIntros "!>" (e2 σ2 efs Hstep).
-  rewrite Hexend in Hheap. inv_head_step.
-  iMod (@gen_heap_update with "Hsi Hl") as "[Hsi Hl]".
-  iMod (update_no_step_enough_fuel _ _ ∅ with "HfuelS Hmi") as (δ2 ℓ) "([%Hlabels %Hvse] & Hfuel & Hmod)" =>//.
-  { by intros ?%dom_empty_inv_L. }
-  { set_solver. }
-  { rewrite Hexend. apply head_locale_step. by econstructor. }
-  iModIntro; iExists _,_.
-  rewrite Hexend //=. iFrame "Hsi Hmod".
-  do 2 (iSplit=>//).
-  iApply "HΦ". iFrame. iApply (has_fuels_proper with "Hfuel") =>//.
-  rewrite map_filter_id //. intros ???%elem_of_dom_2; set_solver.
-Qed.
+(* Lemma wp_load_nostep s tid E l q v fs: *)
+(*   fs ≠ ∅ -> *)
+(*   {{{ ▷ l ↦{q} v ∗ has_fuels_S tid fs }}} Load (Val $ LitV $ LitLoc l) @ s; tid; E {{{ RET v; l ↦{q} v ∗ has_fuels tid fs }}}. *)
+(* Proof. *)
+(*   iIntros (? Φ) "[>Hl HfuelS] HΦ". iApply wp_lift_atomic_head_step_no_fork; auto. *)
+(*   iIntros (extr atr K tp1 tp2 σ1 Hval Hexend Hloc) "(% & Hsi & Hmi) !>". *)
+(*   iDestruct (@gen_heap_valid with "Hsi Hl") as %Hheap. *)
+(*   iSplit; first by rewrite Hexend // in Hheap;  eauto. iIntros "!>" (e2 σ2 efs Hstep). *)
+(*   rewrite Hexend in Hheap. inv_head_step. *)
+(*   iMod (update_no_step_enough_fuel _ _ ∅ with "HfuelS Hmi") as (δ2 ℓ) "([%Hlabels %Hvse] & Hfuel & Hmod)" =>//. *)
+(*   { by intros ?%dom_empty_inv_L. } *)
+(*   { set_solver. } *)
+(*   { rewrite Hexend. apply head_locale_step. by econstructor. } *)
+(*   iModIntro; iExists _,_. *)
+(*   rewrite Hexend //=. iFrame "Hsi Hmod". *)
+(*   do 2 (iSplit=>//). *)
+(*   iApply "HΦ". iFrame. iApply (has_fuels_proper with "Hfuel") =>//. *)
+(*   rewrite map_filter_id //. intros ???%elem_of_dom_2; set_solver. *)
+(* Qed. *)
 
-(* WIP solution for generic fuel-handling *)
-Definition sswp (s : stuckness) E e1 (Φ : expr → iProp Σ) : iProp Σ :=
-  match to_val e1 with
-  | Some v => |={E}=> Φ (of_val v)
-  | None => ∀ σ1,
-      gen_heap_interp σ1.(heap) ={E,∅}=∗
-       ⌜if s is NotStuck then reducible e1 σ1 else True⌝ ∗
-       ∀ e2 σ2 efs,
-         ⌜prim_step e1 σ1 e2 σ2 efs⌝ ={∅}▷=∗ |={∅,E}=>
-         gen_heap_interp σ2.(heap) ∗ Φ e2 ∗ ⌜efs = []⌝
-  end%I.
 
-Lemma wp_store s tid E l v' v :
+Lemma wp_store s E l v' v (Φ : expr → iProp Σ) :
   ▷ l ↦ v' -∗
-  sswp s E (Store (Val $ LitV (LitLoc l)) (Val v))
-            (λ w, ⌜w = LitV LitUnit⌝ ∗ l ↦ v ).
+  ▷ (l ↦ v -∗ Φ $ LitV LitUnit) -∗
+  sswp s E (Store (Val $ LitV (LitLoc l)) (Val v)) Φ.
 Proof.
-  iIntros ">Hl". simpl.
+  iIntros ">Hl HΦ". simpl.
   iIntros (σ1) "Hsi".
   iDestruct (gen_heap_valid with "Hsi Hl") as %Hheap.
   iApply fupd_mask_intro; [set_solver|]. iIntros "Hclose".
@@ -1091,53 +665,32 @@ Proof.
   iMod (@gen_heap_update with "Hsi Hl") as "[Hsi Hl]".
   iFrame.
   apply head_reducible_prim_step in Hstep; [|by eauto].
-  inv_head_step. iFrame. done.
+  inv_head_step. iFrame. iModIntro. iSplit; [|done]. by iApply "HΦ".
 Qed.
 
-Lemma wp_nostep s tid E e fs Φ :
-  TCEq (to_val e) None →
-  fs ≠ ∅ →
-  sswp s E e (λ e', has_fuels tid fs -∗ WP e' @ s; tid; E {{ Φ }} ) -∗
-  has_fuels_S tid fs -∗
-  WP e @ s; tid; E {{ Φ }}.
-Proof.
-  iIntros (Hval ?) "Hwp HfuelS".
-  rewrite wp_unfold /wp_pre /sswp /= Hval.
-  iIntros (extr atr K tp1 tp2 σ1 Hvalid Hloc Hends) "(%Hvalid' & Hsi & Hmi)".
-  rewrite Hends.
-  iMod ("Hwp" with "Hsi") as (Hred) "Hwp".
-  iModIntro. iSplit; [done|].
-  iIntros (e2 σ2 efs Hstep). simpl in *.
-  iMod ("Hwp" with "[//]") as "Hwp".
-  iIntros "!>!>". iMod "Hwp". iIntros "!>".
-  iApply step_fupdN_intro; [done|]. iIntros "!>". iMod "Hwp".
-  iMod (update_no_step_enough_fuel extr atr ∅ with "HfuelS [Hmi]") as (δ2 ℓ) "([%Hlabels %Hvse] & Hfuel & Hmod)" =>//.
-  { by intros ?%dom_empty_inv_L. }
-  { set_solver. }
-  { rewrite Hends  -Hloc. eapply locale_step_atomic; eauto. by apply fill_step. }
-  { by rewrite Hends. }
-  iIntros "!>".
-  iDestruct "Hwp" as "[Hsi [Hwp ->]]".
-  iExists _, _. iFrame. iSplit; [done|].
-  rewrite map_filter_id //; [|intros ???%elem_of_dom_2; set_solver].
-  iDestruct ("Hwp" with "Hfuel") as "Hwp". iFrame. done.
-Qed.
-
-Lemma sswp_wand s e E (Φ Ψ : expr → iProp Σ) :
-  (∀ e, Φ e -∗ Ψ e) -∗ sswp s E e Φ -∗ sswp s E e Ψ.
-Proof.
-  iIntros "HΦΨ HΦ".
-  rewrite /sswp.
-  destruct (to_val e); [by iApply "HΦΨ"|].
-  iIntros (?) "H".
-  iMod ("HΦ" with "H") as "[%Hs HΦ]".
-  iModIntro. iSplit; [done|].
-  iIntros (????).
-  iDestruct ("HΦ" with "[//]") as "HΦ".
-  iMod "HΦ". iIntros "!>!>". iMod "HΦ". iIntros "!>". iMod "HΦ" as "(?&?&?)".
-  iIntros "!>". iFrame.
-  by iApply "HΦΨ".
-Qed.
+(* Lemma wp_store_nostep s tid E l v' v fs: *)
+(*   fs ≠ ∅ -> *)
+(*   {{{ ▷ l ↦ v' ∗ has_fuels_S tid fs }}} *)
+(*     Store (Val $ LitV (LitLoc l)) (Val v) @ s; tid; E *)
+(*   {{{ RET LitV LitUnit; l ↦ v ∗ has_fuels tid fs }}}. *)
+(* Proof. *)
+(*   iIntros (? Φ) "[>Hl HfuelS] HΦ". *)
+(*   iApply wp_lift_atomic_head_step_no_fork; auto. *)
+(*   iIntros (extr atr K tp1 tp2 σ1 Hval Hexend Hloc) "(% & Hsi & Hmi) !>". *)
+(*   iDestruct (@gen_heap_valid with "Hsi Hl") as %Hheap. *)
+(*   iSplit; first by rewrite Hexend // in Hheap;  eauto. iIntros "!>" (e2 σ2 efs Hstep). *)
+(*   rewrite Hexend in Hheap. inv_head_step. *)
+(*   iMod (@gen_heap_update with "Hsi Hl") as "[Hsi Hl]". *)
+(*   iMod (update_no_step_enough_fuel _ _ ∅ with "HfuelS Hmi") as (δ2 ℓ) "([%Hlabels %Hvse] & Hfuel & Hmod)" =>//. *)
+(*   { by intros ?%dom_empty_inv_L. } *)
+(*   { set_solver. } *)
+(*   { rewrite Hexend. apply head_locale_step. by econstructor. } *)
+(*   iModIntro; iExists _,_. *)
+(*   rewrite Hexend //=. iFrame "Hsi Hmod". *)
+(*   do 2 (iSplit=>//). *)
+(*   iApply "HΦ". iFrame. iApply (has_fuels_proper with "Hfuel") =>//. *)
+(*   rewrite map_filter_id //. intros ???%elem_of_dom_2; set_solver. *)
+(* Qed. *)
 
 (* Sanity check for sswp *)
 Lemma wp_store_nostep_alt s tid E l v' v fs:
@@ -1147,168 +700,289 @@ Lemma wp_store_nostep_alt s tid E l v' v fs:
     {{ λ w, ⌜w = LitV LitUnit⌝ ∗ l ↦ v ∗ has_fuels tid fs}}.
 Proof.
   iIntros (?) ">Hl Hf".
-  iApply (wp_nostep with "[Hl]"); [done| |].
-  { iApply sswp_wand; [|by iApply wp_store].
-    iIntros (e) "[-> Hl] Hf". iApply wp_value. by iFrame. }
+  iApply (wp_step_fuel with "[Hf]"); [done|done|].
+  iApply (wp_store with "Hl").
+  iIntros "!> Hl Hf". iApply wp_value. by iFrame.
+Qed.
+
+(* Lemma wp_store_step_singlerole s tid ρ (f1 f2: nat) fr s1 s2 E l v' v : *)
+(*   f2 ≤ LM.(lm_fl) s2 -> fmtrans M s1 (Some ρ) s2 -> *)
+(*   live_roles _ s2 ⊆ live_roles _ s1 -> *)
+(*   {{{ ▷ l ↦ v' ∗ ▷ frag_model_is s1 ∗ ▷ has_fuel tid ρ f1 ∗ ▷ frag_free_roles_are fr }}} *)
+(*     Store (Val $ LitV $ LitLoc l) (Val v) @ s; tid; E *)
+(*   {{{ RET LitV LitUnit; l ↦ v ∗ frag_model_is s2 ∗ frag_free_roles_are fr ∗ *)
+(*       (if decide (ρ ∈ live_roles M s2) then has_fuel tid ρ f2 else tid ↦M ∅ ) }}}. *)
+(* Proof. *)
+(*   iIntros (Hfl Htrans ? Φ) "(>Hl & >Hst & >Hfuel1 & > Hfr) HΦ". *)
+(*   iApply wp_lift_atomic_head_step_no_fork; auto. *)
+(*   iIntros (extr atr K tp1 tp2 σ1 Hval Hexend Hloc) "(% & Hsi & Hmi) !>". *)
+(*   iDestruct (@gen_heap_valid with "Hsi Hl") as %Hheap. *)
+(*   iSplit; first by rewrite Hexend // in Hheap;  eauto. *)
+(*   iIntros "!>" (e2 σ2 efs Hstep). *)
+(*   rewrite Hexend in Hheap. inv_head_step. *)
+(*   iDestruct (model_agree' with "Hmi Hst") as %Hmeq. *)
+(*   rewrite has_fuel_fuels Hexend. *)
+(*   iMod (@gen_heap_update with "Hsi Hl") as "[Hsi Hl]". *)
+(*   iMod (update_step_still_alive _ _ _ _ _ _ _ _ _ *)
+(*             (if decide (ρ ∈ live_roles M s2) then {[ ρ := f2 ]} else ∅) *)
+(*             with "Hfuel1 Hst Hmi Hfr") as *)
+(*         (δ2 ℓ) "([%Hlab %Hvse] & Hfuel & Hst & Hfr & Hmod)"; eauto. *)
+(*   - set_solver. *)
+(*   - destruct (decide (ρ ∈ live_roles M s2)); apply head_locale_step; econstructor =>//. *)
+(*   - destruct (decide (ρ ∈ live_roles M s2)). *)
+(*     + split; first by intros _; rewrite lookup_singleton /=; lia. *)
+(*       split; first set_solver. *)
+(*       split; first set_solver. *)
+(*       split; first (intros ρ' Hin; set_solver). *)
+(*       split; set_solver. *)
+(*     + repeat (split; set_solver). *)
+(*   - iModIntro; iExists δ2, ℓ. iSplit. *)
+(*     { iPureIntro. simpl in *. split =>//. } *)
+(*     iFrame. *)
+(*     iSplit; first done. *)
+(*     iApply "HΦ". iFrame. *)
+(*     replace (fr ∖ (live_roles M s2 ∖ live_roles M s1)) *)
+(*       with fr; [iFrame|set_solver]. *)
+(*     destruct (decide (ρ ∈ live_roles M s2)). *)
+(*     + rewrite has_fuel_fuels //. *)
+(*     + iDestruct "Hfuel" as "[?_]". rewrite dom_empty_L //. *)
+(* Qed. *)
+
+Lemma wp_cmpxchg_fail s E l q v' v1 v2 (Φ : expr → iProp Σ) :
+  v' ≠ v1 → vals_compare_safe v' v1 →
+  ▷ l ↦{q} v' -∗
+  ▷ (l ↦{q} v' -∗ Φ $ PairV v' (LitV $ LitBool false)) -∗
+  sswp s E (CmpXchg (Val $ LitV $ LitLoc l) (Val v1) (Val v2)) Φ.
+Proof.
+  iIntros (??) ">Hl HΦ". simpl.
+  iIntros (σ1) "Hsi".
+  iDestruct (gen_heap_valid with "Hsi Hl") as %Hheap.
+  iApply fupd_mask_intro; [set_solver|]. iIntros "Hclose".
+  iSplit.
+  { destruct s; [|done]. iPureIntro. apply head_prim_reducible. by eauto. }
+  iIntros (e2 σ2 efs Hstep). iIntros "!>!>!>".
+  iMod "Hclose".
   iFrame.
+  apply head_reducible_prim_step in Hstep; [|by eauto].
+  inv_head_step.
+  rewrite bool_decide_false //. iFrame. iModIntro.
+  iSplit; [|done].
+  by iApply "HΦ".
 Qed.
 
-Lemma wp_store_step_singlerole s tid ρ (f1 f2: nat) fr s1 s2 E l v' v :
-  f2 ≤ LM.(lm_fl) s2 -> fmtrans M s1 (Some ρ) s2 ->
-  live_roles _ s2 ⊆ live_roles _ s1 ->
-  {{{ ▷ l ↦ v' ∗ ▷ frag_model_is s1 ∗ ▷ has_fuel tid ρ f1 ∗ ▷ frag_free_roles_are fr }}}
-    Store (Val $ LitV $ LitLoc l) (Val v) @ s; tid; E
-  {{{ RET LitV LitUnit; l ↦ v ∗ frag_model_is s2 ∗ frag_free_roles_are fr ∗
-      (if decide (ρ ∈ live_roles M s2) then has_fuel tid ρ f2 else tid ↦M ∅ ) }}}.
+(* Lemma wp_cmpxchg_fail_step_singlerole s tid ρ (f1 f2: nat) fr s1 s2 E l q v' v1 v2: *)
+(*   v' ≠ v1 → vals_compare_safe v' v1 → f2 ≤ LM.(lm_fl) s2 -> M.(fmtrans) s1 (Some ρ) s2 -> *)
+(*   live_roles _ s2 ⊆ live_roles _ s1 -> *)
+(*   {{{ ▷ l ↦{q} v' ∗ ▷ frag_model_is s1 ∗ ▷ has_fuel tid ρ f1 ∗ ▷ frag_free_roles_are fr }}} CmpXchg (Val $ LitV $ LitLoc l) (Val v1) (Val v2) @ s; tid; E *)
+(*   {{{ RET PairV v' (LitV $ LitBool false); l ↦{q} v' ∗ frag_model_is s2 ∗ frag_free_roles_are fr ∗ *)
+(*       (if decide (ρ ∈ live_roles M s2) then has_fuel tid ρ f2 else tid ↦M ∅ ) }}}. *)
+(* Proof. *)
+(*   iIntros (?? Hfl Htrans ? Φ) "(>Hl & >Hst & >Hfuel1 & > Hfr) HΦ". iApply wp_lift_atomic_head_step_no_fork; auto. *)
+(*   iIntros (extr atr K tp1 tp2 σ1 Hval Hexend Hloc) "(% & Hsi & Hmi) !>". *)
+(*   iDestruct (@gen_heap_valid with "Hsi Hl") as %Hheap. *)
+(*   iSplit; first by rewrite Hexend // in Hheap;  eauto. iIntros "!>" (e2 σ2 efs Hstep). *)
+(*   rewrite Hexend in Hheap. inv_head_step. *)
+(*   iDestruct (model_agree' with "Hmi Hst") as %Hmeq. *)
+(*   rewrite bool_decide_false //. *)
+(*   rewrite has_fuel_fuels Hexend. *)
+(*   iMod (update_step_still_alive _ _ _ _ _ _ _ _ _ *)
+(*             (if decide (ρ ∈ live_roles M s2) then {[ ρ := f2 ]} else ∅) *)
+(*             with "Hfuel1 Hst Hmi Hfr") as *)
+(*         (δ2 ℓ) "([%Hlab %Hvse] & Hfuel & Hst & Hfr & Hmod)"; eauto. *)
+(*   - set_solver. *)
+(*   - destruct (decide (ρ ∈ live_roles M s2)); apply head_locale_step; econstructor =>//. *)
+(*   - destruct (decide (ρ ∈ live_roles M s2)). *)
+(*     + split; first by intros _; rewrite lookup_singleton /=; lia. *)
+(*       split; first set_solver. *)
+(*       split; first set_solver. *)
+(*       split; first (intros ρ' Hin; set_solver). *)
+(*       split; set_solver. *)
+(*     + repeat (split; set_solver). *)
+(*   - rewrite -> bool_decide_eq_false_2 in *; eauto. *)
+(*     iModIntro; iExists δ2, ℓ. iSplit. *)
+(*     { iPureIntro. simpl in *. split =>//. } *)
+(*     iFrame. *)
+(*     iSplit; first done. iApply "HΦ". iFrame. *)
+(*     replace (fr ∖ (live_roles M s2 ∖ live_roles M s1)) with fr; [iFrame|set_solver]. *)
+(*     destruct (decide (ρ ∈ live_roles M s2)). *)
+(*     + rewrite has_fuel_fuels //. *)
+(*     + iDestruct "Hfuel" as "[?_]". rewrite dom_empty_L //. *)
+(* Qed. *)
+
+Lemma wp_cmpxchg_suc s E l v' v1 v2 (Φ : expr → iProp Σ) :
+  v' = v1 → vals_compare_safe v' v1 →
+  ▷ l ↦ v' -∗
+  ▷ (l ↦ v2 -∗ Φ $ PairV v' (LitV $ LitBool true)) -∗
+  sswp s E (CmpXchg (Val $ LitV $ LitLoc l) (Val v1) (Val v2)) Φ.
 Proof.
-  iIntros (Hfl Htrans ? Φ) "(>Hl & >Hst & >Hfuel1 & > Hfr) HΦ".
-  iApply wp_lift_atomic_head_step_no_fork; auto.
-  iIntros (extr atr K tp1 tp2 σ1 Hval Hexend Hloc) "(% & Hsi & Hmi) !>".
-  iDestruct (@gen_heap_valid with "Hsi Hl") as %Hheap.
-  iSplit; first by rewrite Hexend // in Hheap;  eauto.
-  iIntros "!>" (e2 σ2 efs Hstep).
-  rewrite Hexend in Hheap. inv_head_step.
-  iDestruct (model_agree' with "Hmi Hst") as %Hmeq.
-  rewrite has_fuel_fuels Hexend.
+  iIntros (??) ">Hl HΦ". simpl.
+  iIntros (σ1) "Hsi".
+  iDestruct (gen_heap_valid with "Hsi Hl") as %Hheap.
+  iApply fupd_mask_intro; [set_solver|]. iIntros "Hclose".
+  iSplit.
+  { destruct s; [|done]. iPureIntro. apply head_prim_reducible. by eauto. }
+  iIntros (e2 σ2 efs Hstep). iIntros "!>!>!>".
   iMod (@gen_heap_update with "Hsi Hl") as "[Hsi Hl]".
-  iMod (update_step_still_alive _ _ _ _ _ _ _ _ _
-            (if decide (ρ ∈ live_roles M s2) then {[ ρ := f2 ]} else ∅)
-            with "Hfuel1 Hst Hmi Hfr") as
-        (δ2 ℓ) "([%Hlab %Hvse] & Hfuel & Hst & Hfr & Hmod)"; eauto.
-  - set_solver.
-  - destruct (decide (ρ ∈ live_roles M s2)); apply head_locale_step; econstructor =>//.
-  - destruct (decide (ρ ∈ live_roles M s2)).
-    + split; first by intros _; rewrite lookup_singleton /=; lia.
-      split; first set_solver.
-      split; first set_solver.
-      split; first (intros ρ' Hin; set_solver).
-      split; set_solver.
-    + repeat (split; set_solver).
-  - iModIntro; iExists δ2, ℓ. iSplit.
-    { iPureIntro. simpl in *. split =>//. }
-    iFrame.
-    iSplit; first done.
-    iApply "HΦ". iFrame.
-    replace (fr ∖ (live_roles M s2 ∖ live_roles M s1))
-      with fr; [iFrame|set_solver].
-    destruct (decide (ρ ∈ live_roles M s2)).
-    + rewrite has_fuel_fuels //.
-    + iDestruct "Hfuel" as "[?_]". rewrite dom_empty_L //.
+  iMod "Hclose".
+  iFrame.
+  apply head_reducible_prim_step in Hstep; [|by eauto].
+  inv_head_step.
+  rewrite bool_decide_true //. iFrame. iModIntro.
+  iSplit; [|done].
+  by iApply "HΦ".
 Qed.
 
-Lemma wp_cmpxchg_fail_step_singlerole s tid ρ (f1 f2: nat) fr s1 s2 E l q v' v1 v2:
-  v' ≠ v1 → vals_compare_safe v' v1 → f2 ≤ LM.(lm_fl) s2 -> M.(fmtrans) s1 (Some ρ) s2 ->
-  live_roles _ s2 ⊆ live_roles _ s1 ->
-  {{{ ▷ l ↦{q} v' ∗ ▷ frag_model_is s1 ∗ ▷ has_fuel tid ρ f1 ∗ ▷ frag_free_roles_are fr }}} CmpXchg (Val $ LitV $ LitLoc l) (Val v1) (Val v2) @ s; tid; E
-  {{{ RET PairV v' (LitV $ LitBool false); l ↦{q} v' ∗ frag_model_is s2 ∗ frag_free_roles_are fr ∗
-      (if decide (ρ ∈ live_roles M s2) then has_fuel tid ρ f2 else tid ↦M ∅ ) }}}.
-Proof.
-  iIntros (?? Hfl Htrans ? Φ) "(>Hl & >Hst & >Hfuel1 & > Hfr) HΦ". iApply wp_lift_atomic_head_step_no_fork; auto.
-  iIntros (extr atr K tp1 tp2 σ1 Hval Hexend Hloc) "(% & Hsi & Hmi) !>".
-  iDestruct (@gen_heap_valid with "Hsi Hl") as %Hheap.
-  iSplit; first by rewrite Hexend // in Hheap;  eauto. iIntros "!>" (e2 σ2 efs Hstep).
-  rewrite Hexend in Hheap. inv_head_step.
-  iDestruct (model_agree' with "Hmi Hst") as %Hmeq.
-  rewrite bool_decide_false //.
-  rewrite has_fuel_fuels Hexend.
-  iMod (update_step_still_alive _ _ _ _ _ _ _ _ _
-            (if decide (ρ ∈ live_roles M s2) then {[ ρ := f2 ]} else ∅)
-            with "Hfuel1 Hst Hmi Hfr") as
-        (δ2 ℓ) "([%Hlab %Hvse] & Hfuel & Hst & Hfr & Hmod)"; eauto.
-  - set_solver.
-  - destruct (decide (ρ ∈ live_roles M s2)); apply head_locale_step; econstructor =>//.
-  - destruct (decide (ρ ∈ live_roles M s2)).
-    + split; first by intros _; rewrite lookup_singleton /=; lia.
-      split; first set_solver.
-      split; first set_solver.
-      split; first (intros ρ' Hin; set_solver).
-      split; set_solver.
-    + repeat (split; set_solver).
-  - rewrite -> bool_decide_eq_false_2 in *; eauto.
-    iModIntro; iExists δ2, ℓ. iSplit.
-    { iPureIntro. simpl in *. split =>//. }
-    iFrame.
-    iSplit; first done. iApply "HΦ". iFrame.
-    replace (fr ∖ (live_roles M s2 ∖ live_roles M s1)) with fr; [iFrame|set_solver].
-    destruct (decide (ρ ∈ live_roles M s2)).
-    + rewrite has_fuel_fuels //.
-    + iDestruct "Hfuel" as "[?_]". rewrite dom_empty_L //.
-Qed.
+(* Lemma wp_step_model_singlerole s tid ρ (f1 : nat) fs fr s1 s2 E e Φ : *)
+(*   TCEq (to_val e) None → *)
+(*   ρ ∉ dom fs → *)
+(*   fmtrans M s1 (Some ρ) s2 → *)
+(*   ▷ frag_model_is s1 -∗ ▷ has_fuel tid ρ f1 -∗ *)
+(*   ▷ frag_free_roles_are fr -∗ *)
+(*   sswp s E e (λ e', frag_model_is s2 -∗ frag_free_roles_are fr -∗ *)
+(*                     has_fuels tid ({[ρ:=(LM.(lm_fl) s2)]} ∪ fs) -∗ *)
+(*                     WP e' @ s; tid; E {{ Φ }} ) -∗ *)
+(*   WP e @ s; tid; E {{ Φ }}. *)
+(* Proof. *)
+(*   iIntros (Hval Hdom Htrans) ">Hst >Hfuel1 >Hfr Hwp". *)
+(*   rewrite wp_unfold /wp_pre. *)
+(*   rewrite /sswp. simpl. rewrite Hval. *)
+(*   iIntros (extr atr K tp1 tp2 σ1 Hvalid Hloc Hexend) "(% & Hsi & Hmi)". *)
+(*   iMod ("Hwp" with "Hsi") as (Hred) "Hwp". *)
+(*   iIntros "!>". *)
+(*   iSplitR; [by rewrite Hexend in Hred|]. *)
+(*   iIntros (????). *)
+(*   rewrite Hexend. *)
+(*   iMod ("Hwp" with "[//]") as "Hwp". iIntros "!>!>". iMod "Hwp". iIntros "!>". *)
+(*   iApply step_fupdN_intro; [done|]. iIntros "!>". *)
+(*   iMod "Hwp" as "[Hσ [Hwp ->]]". *)
+(*   iDestruct (model_agree' with "Hmi Hst") as %Hmeq. *)
+(*   iFrame. *)
+(*   rewrite /trace_ends_in in Hexend. *)
+(*   rewrite -Hexend. *)
+(*   iMod (update_model_step with "Hfuel1 Hst Hmi") as *)
+(*     (δ2 Hvse) "(Hfuel & Hst & Hmod)"; eauto. *)
+(*   - rewrite -Hloc. *)
+(*     eapply locale_step_atomic; eauto. *)
+(*     by apply fill_step. *)
+(*   - iModIntro; iExists δ2, (Take_step ρ tid). *)
+(*     rewrite big_sepL_nil. iFrame. *)
+(*     iSplit. *)
+(*     { iPureIntro. simpl in *. naive_solver. } *)
+(*     iDestruct ("Hwp" with "Hst Hfr Hfuel") as "Hwp". by iFrame. *)
+(* Qed. *)
 
-Lemma wp_cmpxchg_suc_step_singlerole_keep_dead  s tid ρ (f1 f2: nat) fr s1 s2 E l v' v1 v2:
+(* Sanity Check *)
+Lemma wp_cmpxchg_suc_step_singlerole_keep_dead_alt s tid ρ (f1: nat) fr s1 s2 E l v' v1 v2:
   ρ ∉ live_roles _ s2 →
-  v' = v1 → vals_compare_safe v' v1 → f2 < f1 -> M.(fmtrans) s1 (Some ρ) s2 ->
+  v' = v1 → vals_compare_safe v' v1 → M.(fmtrans) s1 (Some ρ) s2 ->
   live_roles _ s2 ⊆ live_roles _ s1 ->
   {{{ ▷ l ↦ v' ∗ ▷ frag_model_is s1 ∗ ▷ has_fuel tid ρ f1 ∗ ▷ frag_free_roles_are fr }}}
     CmpXchg (Val $ LitV $ LitLoc l) (Val v1) (Val v2) @ s; tid; E
   {{{ RET PairV v' (LitV $ LitBool true); l ↦ v2 ∗ frag_model_is s2 ∗ frag_free_roles_are fr ∗
-      has_fuel tid ρ f2 }}}.
+      has_fuel tid ρ (lm_fl LM s2) }}}.
 Proof.
-  iIntros (??? Hfl Htrans ? Φ) "(>Hl & >Hst & >Hfuel1 & >Hfr) HΦ".
-  iApply wp_lift_atomic_head_step_no_fork; auto.
-  iIntros (extr atr K tp1 tp2 σ1 Hval Hexend Hloc) "(% & Hsi & Hmi) !>".
-  iDestruct (@gen_heap_valid with "Hsi Hl") as %Hheap.
-  iSplit; first by rewrite Hexend // in Hheap;  eauto. iIntros "!>" (e2 σ2 efs Hstep).
-  rewrite Hexend in Hheap. inv_head_step.
-  iDestruct (model_agree' with "Hmi Hst") as %Hmeq.
-  rewrite bool_decide_true //.
-  iMod (@gen_heap_update with "Hsi Hl") as "[Hsi Hl]".
-  rewrite has_fuel_fuels Hexend.
-  iMod (update_step_still_alive _ _ _ _ _ _ _ _ _ {[ ρ := f2 ]} with "Hfuel1 Hst Hmi Hfr") as
-        (δ2 ℓ) "([%Hlab %Hvse] & Hfuel & Hst & Hfr & Hmod)"; eauto.
-  - set_solver.
-  - apply head_locale_step; econstructor =>//.
-  - repeat (split; try done); [|set_solver|set_solver|set_solver| set_solver |].
-    + intros ??. rewrite !lookup_singleton /=. lia.
-    + rewrite dom_singleton singleton_subseteq_l. simplify_eq.
-      destruct (decide (ρ ∈ live_roles _ (trace_last atr))); set_solver.
-  - rewrite -> bool_decide_eq_true_2 in *; eauto.
-    iModIntro; iExists δ2, ℓ. iSplit.
-    { iPureIntro. simpl in *. split =>//. }
-    iFrame. iSplit; first done. iApply "HΦ". iFrame.
-    replace (fr ∖ (live_roles M s2 ∖ live_roles M s1)) with fr; [iFrame|set_solver].
-    by rewrite has_fuel_fuels.
+  iIntros (??? Htrans ? Φ) "(>Hl & >Hst & >Hfuel1 & >Hfr) HΦ".
+  iApply (wp_step_model_singlerole with "Hst Hfuel1 Hfr"); [done..|].
+  iApply (wp_cmpxchg_suc with "Hl"); [done..|].
+  iIntros "!> Hl Hs Hfr Hfuel2".
+  iApply wp_value. iApply "HΦ". iFrame.
 Qed.
 
-Lemma wp_cmpxchg_suc_step_singlerole s tid ρ (f1 f2: nat) fr s1 s2 E l v' v1 v2:
-  v' = v1 → vals_compare_safe v' v1 → f2 ≤ LM.(lm_fl) s2 -> M.(fmtrans) s1 (Some ρ) s2 ->
+(* Lemma wp_cmpxchg_suc_step_singlerole_keep_dead  s tid ρ (f1 f2: nat) fr s1 s2 E l v' v1 v2: *)
+(*   ρ ∉ live_roles _ s2 → *)
+(*   v' = v1 → vals_compare_safe v' v1 → f2 < f1 -> M.(fmtrans) s1 (Some ρ) s2 -> *)
+(*   live_roles _ s2 ⊆ live_roles _ s1 -> *)
+(*   {{{ ▷ l ↦ v' ∗ ▷ frag_model_is s1 ∗ ▷ has_fuel tid ρ f1 ∗ ▷ frag_free_roles_are fr }}} *)
+(*     CmpXchg (Val $ LitV $ LitLoc l) (Val v1) (Val v2) @ s; tid; E *)
+(*   {{{ RET PairV v' (LitV $ LitBool true); l ↦ v2 ∗ frag_model_is s2 ∗ frag_free_roles_are fr ∗ *)
+(*       has_fuel tid ρ f2 }}}. *)
+(* Proof. *)
+(*   iIntros (??? Hfl Htrans ? Φ) "(>Hl & >Hst & >Hfuel1 & >Hfr) HΦ". *)
+(*   iApply wp_lift_atomic_head_step_no_fork; auto. *)
+(*   iIntros (extr atr K tp1 tp2 σ1 Hval Hexend Hloc) "(% & Hsi & Hmi) !>". *)
+(*   iDestruct (@gen_heap_valid with "Hsi Hl") as %Hheap. *)
+(*   iSplit; first by rewrite Hexend // in Hheap;  eauto. iIntros "!>" (e2 σ2 efs Hstep). *)
+(*   rewrite Hexend in Hheap. inv_head_step. *)
+(*   iDestruct (model_agree' with "Hmi Hst") as %Hmeq. *)
+(*   rewrite bool_decide_true //. *)
+(*   iMod (@gen_heap_update with "Hsi Hl") as "[Hsi Hl]". *)
+(*   rewrite has_fuel_fuels Hexend. *)
+(*   iMod (update_step_still_alive _ _ _ _ _ _ _ _ _ {[ ρ := f2 ]} with "Hfuel1 Hst Hmi Hfr") as *)
+(*         (δ2 ℓ) "([%Hlab %Hvse] & Hfuel & Hst & Hfr & Hmod)"; eauto. *)
+(*   - set_solver. *)
+(*   - apply head_locale_step; econstructor =>//. *)
+(*   - repeat (split; try done); [|set_solver|set_solver|set_solver| set_solver |]. *)
+(*     + intros ??. rewrite !lookup_singleton /=. lia. *)
+(*     + rewrite dom_singleton singleton_subseteq_l. simplify_eq. *)
+(*       destruct (decide (ρ ∈ live_roles _ (trace_last atr))); set_solver. *)
+(*   - rewrite -> bool_decide_eq_true_2 in *; eauto. *)
+(*     iModIntro; iExists δ2, ℓ. iSplit. *)
+(*     { iPureIntro. simpl in *. split =>//. } *)
+(*     iFrame. iSplit; first done. iApply "HΦ". iFrame. *)
+(*     replace (fr ∖ (live_roles M s2 ∖ live_roles M s1)) with fr; [iFrame|set_solver]. *)
+(*     by rewrite has_fuel_fuels. *)
+(* Qed. *)
+
+(* OBS: tid ↦M ∅ vs has_fuels tid ∅ *)
+Lemma wp_cmpxchg_suc_step_singlerole_alt s tid ρ (f1: nat) fr s1 s2 E l v' v1 v2:
+  v' = v1 → vals_compare_safe v' v1 → M.(fmtrans) s1 (Some ρ) s2 ->
   live_roles _ s2 ⊆ live_roles _ s1 ->
   {{{ ▷ l ↦ v' ∗ ▷ frag_model_is s1 ∗ ▷ has_fuel tid ρ f1 ∗ ▷ frag_free_roles_are fr }}}
     CmpXchg (Val $ LitV $ LitLoc l) (Val v1) (Val v2) @ s; tid; E
   {{{ RET PairV v' (LitV $ LitBool true); l ↦ v2 ∗ frag_model_is s2 ∗ frag_free_roles_are fr ∗
-      (if decide (ρ ∈ live_roles M s2) then has_fuel tid ρ f2 else tid ↦M ∅ ) }}}.
+      (if decide (ρ ∈ live_roles M s2) then has_fuel tid ρ (lm_fl LM s2) else has_fuels tid ∅ ) }}}.
 Proof.
-  iIntros (?? Hfl Htrans ? Φ) "(>Hl & >Hst & >Hfuel1 & >Hfr) HΦ".
-  iApply wp_lift_atomic_head_step_no_fork; auto.
-  iIntros (extr atr K tp1 tp2 σ1 Hval Hexend Hloc) "(% & Hsi & Hmi) !>".
-  iDestruct (@gen_heap_valid with "Hsi Hl") as %Hheap.
-  iSplit; first by rewrite Hexend // in Hheap;  eauto. iIntros "!>" (e2 σ2 efs Hstep).
-  rewrite Hexend in Hheap. inv_head_step.
-  iDestruct (model_agree' with "Hmi Hst") as %Hmeq.
-  rewrite bool_decide_true //.
-  iMod (@gen_heap_update with "Hsi Hl") as "[Hsi Hl]".
-  rewrite has_fuel_fuels Hexend.
-  iMod (update_step_still_alive _ _ _ _ _ _ _ _ _
-            (if decide (ρ ∈ live_roles M s2) then {[ ρ := f2 ]} else ∅)
-            with "Hfuel1 Hst Hmi Hfr") as
-        (δ2 ℓ) "([%Hlab %Hvse] & Hfuel & Hst & Hfr & Hmod)"; eauto.
-  - set_solver.
-  - destruct (decide (ρ ∈ live_roles M s2)); apply head_locale_step; econstructor =>//.
-  - destruct (decide (ρ ∈ live_roles M s2)).
-    + split; first by intros _; rewrite lookup_singleton /=; lia.
-      split; first set_solver.
-      split; first set_solver.
-      split; set_solver.
-    + repeat (split; set_solver).
-  - rewrite -> bool_decide_eq_true_2 in *; eauto.
-    iModIntro; iExists δ2, ℓ. iSplit.
-    { iPureIntro. simpl in *. split =>//. }
-    iFrame. iSplit; first done. iApply "HΦ". iFrame.
-    replace (fr ∖ (live_roles M s2 ∖ live_roles M s1)) with fr; [iFrame|set_solver].
-    destruct (decide (ρ ∈ live_roles M s2)).
-    + rewrite has_fuel_fuels //.
-    + iDestruct "Hfuel" as "[?_]". rewrite dom_empty_L //.
+  iIntros (?? Htrans ? Φ) "(>Hl & >Hst & >Hfuel1 & >Hfr) HΦ".
+  iApply (wp_step_model_singlerole with "Hst Hfuel1 Hfr"); [done..|].
+  iApply (wp_cmpxchg_suc with "Hl"); [done..|].
+  iIntros "!> Hl Hs Hfr Hfuel2".
+  destruct (decide (ρ ∈ live_roles M s2)).
+  { iApply wp_value. iApply "HΦ". iFrame. }
+  iApply pre_step_wp.
+  iMod (has_fuels_dealloc with "Hs Hfuel2") as "[Hs Hfuel2]"; [done|].
+  rewrite delete_insert; [|set_solver].
+  iModIntro. iApply wp_value. iApply "HΦ". iFrame.
 Qed.
+
+(* Lemma wp_cmpxchg_suc_step_singlerole s tid ρ (f1 f2: nat) fr s1 s2 E l v' v1 v2: *)
+(*   v' = v1 → vals_compare_safe v' v1 → f2 ≤ LM.(lm_fl) s2 -> M.(fmtrans) s1 (Some ρ) s2 -> *)
+(*   live_roles _ s2 ⊆ live_roles _ s1 -> *)
+(*   {{{ ▷ l ↦ v' ∗ ▷ frag_model_is s1 ∗ ▷ has_fuel tid ρ f1 ∗ ▷ frag_free_roles_are fr }}} *)
+(*     CmpXchg (Val $ LitV $ LitLoc l) (Val v1) (Val v2) @ s; tid; E *)
+(*   {{{ RET PairV v' (LitV $ LitBool true); l ↦ v2 ∗ frag_model_is s2 ∗ frag_free_roles_are fr ∗ *)
+(*       (if decide (ρ ∈ live_roles M s2) then has_fuel tid ρ f2 else tid ↦M ∅ ) }}}. *)
+(* Proof. *)
+(*   iIntros (?? Hfl Htrans ? Φ) "(>Hl & >Hst & >Hfuel1 & >Hfr) HΦ". *)
+(*   iApply wp_lift_atomic_head_step_no_fork; auto. *)
+(*   iIntros (extr atr K tp1 tp2 σ1 Hval Hexend Hloc) "(% & Hsi & Hmi) !>". *)
+(*   iDestruct (@gen_heap_valid with "Hsi Hl") as %Hheap. *)
+(*   iSplit; first by rewrite Hexend // in Hheap;  eauto. iIntros "!>" (e2 σ2 efs Hstep). *)
+(*   rewrite Hexend in Hheap. inv_head_step. *)
+(*   iDestruct (model_agree' with "Hmi Hst") as %Hmeq. *)
+(*   rewrite bool_decide_true //. *)
+(*   iMod (@gen_heap_update with "Hsi Hl") as "[Hsi Hl]". *)
+(*   rewrite has_fuel_fuels Hexend. *)
+(*   iMod (update_step_still_alive _ _ _ _ _ _ _ _ _ *)
+(*             (if decide (ρ ∈ live_roles M s2) then {[ ρ := f2 ]} else ∅) *)
+(*             with "Hfuel1 Hst Hmi Hfr") as *)
+(*         (δ2 ℓ) "([%Hlab %Hvse] & Hfuel & Hst & Hfr & Hmod)"; eauto. *)
+(*   - set_solver. *)
+(*   - destruct (decide (ρ ∈ live_roles M s2)); apply head_locale_step; econstructor =>//. *)
+(*   - destruct (decide (ρ ∈ live_roles M s2)). *)
+(*     + split; first by intros _; rewrite lookup_singleton /=; lia. *)
+(*       split; first set_solver. *)
+(*       split; first set_solver. *)
+(*       split; set_solver. *)
+(*     + repeat (split; set_solver). *)
+(*   - rewrite -> bool_decide_eq_true_2 in *; eauto. *)
+(*     iModIntro; iExists δ2, ℓ. iSplit. *)
+(*     { iPureIntro. simpl in *. split =>//. } *)
+(*     iFrame. iSplit; first done. iApply "HΦ". iFrame. *)
+(*     replace (fr ∖ (live_roles M s2 ∖ live_roles M s1)) with fr; [iFrame|set_solver]. *)
+(*     destruct (decide (ρ ∈ live_roles M s2)). *)
+(*     + rewrite has_fuel_fuels //. *)
+(*     + iDestruct "Hfuel" as "[?_]". rewrite dom_empty_L //. *)
+(* Qed. *)
 
 (* Lemma wp_faa s E l i1 i2 : *)
 (*   {{{ ▷ l ↦ LitV (LitInt i1) }}} FAA (Val $ LitV $ LitLoc l) (Val $ LitV $ LitInt i2) @ s; E *)
@@ -1320,4 +994,5 @@ Qed.
 (*   iMod (@gen_heap_update with "Hσ Hl") as "[$ Hl]". *)
 (*   iModIntro. iSplit=>//. iFrame. by iApply "HΦ". *)
 (* Qed. *)
+
 End lifting.
